Introduce thread identifier.

theories/zoo/iris/program_logic/adequacy.v
@@ -1,5 +1,7 @@
 From zoo Require Import
   prelude.
+From zoo.common Require Import
+  list.
 From zoo.iris.bi Require Import
   big_op.
 From zoo.iris Require Import
@@ -17,82 +19,87 @@ Section iris_G.
   Implicit Types Φ : val Λ → iProp Σ.
   Implicit Types Φs : list (val Λ → iProp Σ).
 
-  Definition wps es Φs : iProp Σ :=
-    [∗ list] e; Φ ∈ es; Φs,
-      WP e @ ⊤ {{ Φ }}.
+  Definition bwps nt es Φs : iProp Σ :=
+    [∗ list] i ↦ e; Φ ∈ es; Φs,
+      BWP e ∶ nt + i {{ Φ }}.
 
-  #[local] Lemma wp_step e1 σ1 e2 σ2 κ κs es nt Φ :
-    prim_step e1 σ1 κ e2 σ2 es →
+  #[local] Lemma bwp_step tid e1 σ1 e2 σ2 κ κs es nt Φ :
+    prim_step tid e1 σ1 κ e2 σ2 es →
     state_interp nt σ1 (κ ++ κs) -∗
     £ 1 -∗
-    WP e1 @ ⊤ {{ Φ }} -∗
+    BWP e1 ∶ tid {{ Φ }} -∗
       |={⊤}[∅]▷=>
       state_interp (nt + length es) σ2 κs ∗
-      WP e2 @ ⊤ {{ Φ }} ∗
-      wps es (replicate (length es) fork_post).
+      BWP e2 ∶ tid {{ Φ }} ∗
+      bwps nt es (replicate (length es) fork_post).
   Proof.
     iIntros "%Hstep Hσ H£ H".
-    rewrite {1}wp_unfold /wp_pre (val_stuck e1 σ1 κ e2 σ2 es) //.
+    rewrite {1}bwp_unfold /bwp_pre (val_stuck tid e1 σ1 κ e2 σ2 es) //.
     iMod ("H" with "Hσ") as "(_ & H)".
     iMod ("H" with "[//] H£") as "H".
-    iModIntro. iSteps. rewrite /wps big_sepL2_replicate_r //.
+    iModIntro. iSteps. rewrite /bwps big_sepL2_replicate_r //.
   Qed.
-  #[local] Lemma wps_step es1 σ1 es2 σ2 κ κs nt Φs :
+  #[local] Lemma bwps_step es1 σ1 es2 σ2 κ κs Φs :
     step (es1, σ1) κ (es2, σ2) →
-    state_interp nt σ1 (κ ++ κs) -∗
+    state_interp (length es1) σ1 (κ ++ κs) -∗
     £ 1 -∗
-    wps es1 Φs -∗
+    bwps 0 es1 Φs -∗
       |={⊤}[∅]▷=>
-      ∃ n_fork,
-      state_interp (nt + n_fork) σ2 κs ∗
-      wps es2 (Φs ++ replicate n_fork fork_post).
+      state_interp (length es2) σ2 κs ∗
+      bwps 0 es2 (Φs ++ replicate (length es2 - length es1) fork_post).
   Proof.
     iIntros ((i & e1 & e2 & σ2' & es & Hstep & Hes1_lookup & [= -> <-])) "Hσ H£ H".
     iDestruct (big_sepL2_insert_acc_l with "H") as "(%Φ & %HΦs_lookup & He1 & H)"; first done.
-    iMod (wp_step with "Hσ H£ He1") as "He1"; first done.
+    iMod (bwp_step with "Hσ H£ He1") as "He1"; first done.
     do 2 iModIntro.
     iMod "He1" as "(Hσ & He2 & Hes)".
     iDestruct ("H" with "He2") as "H".
-    rewrite (list_insert_id Φs) // big_sepL2_app.
+    rewrite length_app length_insert Nat.add_sub'.
+    rewrite (list_insert_id Φs) // big_sepL2_app length_insert.
     iSteps.
   Qed.
-  #[local] Lemma wps_steps n es1 σ1 es2 σ2 κs1 κs2 nt Φs :
+  #[local] Lemma bwps_steps n es1 σ1 es2 σ2 κs1 κs2 Φs :
     nsteps n (es1, σ1) κs1 (es2, σ2) →
-    state_interp nt σ1 (κs1 ++ κs2) -∗
+    state_interp (length es1) σ1 (κs1 ++ κs2) -∗
     £ n -∗
-    wps es1 Φs -∗
+    bwps 0 es1 Φs -∗
       |={⊤,∅}=> |={∅}▷=>^n |={∅,⊤}=>
-      ∃ n_fork,
-      state_interp (nt + n_fork) σ2 κs2 ∗
-      wps es2 (Φs ++ replicate n_fork fork_post).
+      state_interp (length es2) σ2 κs2 ∗
+      bwps 0 es2 (Φs ++ replicate (length es2 - length es1) fork_post).
   Proof.
-    iInduction n as [| n] "IH" forall (es1 σ1 κs1 κs2 nt Φs) => /=.
+    iInduction n as [| n] "IH" forall (es1 σ1 κs1 κs2 Φs) => /=.
     all: iIntros "%Hsteps Hσ H£s H".
     - invert Hsteps.
-      iExists 0. rewrite Nat.add_0_r right_id. iSteps.
+      rewrite Nat.sub_diag right_id. iSteps.
     - invert Hsteps as [| ? ? (es1' & σ1') ? κ κs1' Hstep Hsteps'].
       rewrite -(assoc (++)).
       iDestruct "H£s" as "(H£ & H£s)".
-      iMod (wps_step with "Hσ H£ H") as "H"; [done.. |].
+      iMod (bwps_step with "Hσ H£ H") as "H"; [done.. |].
       do 3 iModIntro.
       iApply (fupd_trans _ ⊤).
-      iMod "H" as "(%n_fork & Hσ & H)".
+      iMod "H" as "(Hσ & H)".
       iModIntro.
-      iMod ("IH" with "[//] Hσ H£s H") as "H"; [done.. |].
+      iMod ("IH" with "[//] Hσ H£s H") as "H".
       iModIntro.
       iApply (step_fupdN_wand with "H"). iIntros ">H".
-      iDestruct "H" as "(%n_fork' & Hσ & H)".
-      iEval (rewrite -assoc) in "Hσ". rewrite -assoc -replicate_add. iSteps.
+      iDestruct "H" as "(Hσ & H)".
+      rewrite -assoc -replicate_add.
+      assert (length es1' - length es1 + (length es2 - length es1') = length es2 - length es1) as ->.
+      { apply step_length in Hstep.
+        apply nsteps_length in Hsteps'.
+        naive_solver lia.
+      }
+      iSteps.
   Qed.
 
-  #[local] Lemma wp_not_stuck e nt σ κs Φ :
+  #[local] Lemma bwp_not_stuck e tid nt σ κs Φ :
     state_interp nt σ κs -∗
-    WP e {{ Φ }} -∗
+    BWP e ∶ tid {{ Φ }} -∗
       |={⊤, ∅}=>
-      ⌜not_stuck e σ⌝.
+      ⌜not_stuck tid e σ⌝.
   Proof.
     iIntros "Hσ H".
-    rewrite wp_unfold /wp_pre /not_stuck.
+    rewrite bwp_unfold /bwp_pre /not_stuck.
     destruct (to_val e) as [v |] eqn:He.
     - iMod (fupd_mask_subseteq ∅); first done.
       iSteps.
@@ -101,61 +108,80 @@ Section iris_G.
       iSteps.
   Qed.
 
-  #[local] Lemma wps_progress n es1 σ1 e2 es2 σ2 κs1 κs2 nt Φs :
+  #[local] Lemma bwps_progress n es1 σ1 tid e2 es2 σ2 κs1 κs2 Φs :
     nsteps n (es1, σ1) κs1 (es2, σ2) →
-    e2 ∈ es2 →
-    state_interp nt σ1 (κs1 ++ κs2) -∗
+    es2 !! tid = Some e2 →
+    state_interp (length es1) σ1 (κs1 ++ κs2) -∗
     £ n -∗
-    wps es1 Φs -∗
+    bwps 0 es1 Φs -∗
       |={⊤, ∅}=> |={∅}▷=>^n |={∅}=>
-      ⌜not_stuck e2 σ2⌝.
+      ⌜not_stuck tid e2 σ2⌝.
   Proof.
-    iIntros (Hsteps (i & Hes2_lookup)%elem_of_list_lookup) "Hσ H£s He".
-    iMod (wps_steps with "Hσ H£s He") as "H"; [done.. |].
+    iIntros (Hsteps Hes2_lookup) "Hσ H£s He".
+    iMod (bwps_steps with "Hσ H£s He") as "H"; [done.. |].
     iModIntro.
     iApply (step_fupdN_wand with "H").
-    iMod 1 as "(%n_fork & Hσ & H)".
+    iMod 1 as "(Hσ & H)".
     iDestruct (big_sepL2_lookup_Some_l with "H") as %(Φ & Hposts_lookup); first done.
     iDestruct (big_sepL2_lookup with "H") as "H"; [done.. |].
-    iApply (wp_not_stuck with "Hσ H").
+    iApply (bwp_not_stuck with "Hσ H").
   Qed.
 End iris_G.
 
-Lemma wp_progress Λ Σ `{inv_Gpre : !invGpreS Σ} n es1 σ1 es2 σ2 κs :
+Lemma bwp_progress Λ Σ `{inv_Gpre : !invGpreS Σ} n es1 σ1 es2 σ2 κs :
   ( ∀ `{inv_G : !invGS Σ},
     ⊢ |={⊤}=>
-      ∃ state_interp fork_post nt Φs,
+      ∃ state_interp fork_post Φs,
       let iris_G : IrisG Λ Σ := Build_IrisG state_interp fork_post in
-      state_interp nt σ1 κs ∗
-      wps es1 Φs
+      state_interp (length es1) σ1 κs ∗
+      bwps 0 es1 Φs
   ) →
   nsteps n (es1, σ1) κs (es2, σ2) →
-  Forall (λ e2, not_stuck e2 σ2) es2.
+  Foralli (λ tid e2, not_stuck tid e2 σ2) es2.
 Proof.
   intros H Hsteps.
-  apply Forall_forall => e2 He2.
+  apply Foralli_lookup => tid e2 Hlookup.
   eapply uPred.pure_soundness, (step_fupdN_soundness_lc _ n n).
   iIntros "%Hinv_G H£s".
-  iMod H as "(%state_interp & %fork_post & %nt & %Φs & Hσ & H)".
-  iMod (wps_progress (iris_G := Build_IrisG state_interp fork_post) with "[Hσ] H£s H") as "H"; [done.. | |].
+  iMod H as "(%state_interp & %fork_post & %Φs & Hσ & H)".
+  iMod (bwps_progress (iris_G := Build_IrisG state_interp fork_post) with "[Hσ] H£s H") as "H"; [done.. | |].
   { erewrite app_nil_r => //. }
   destruct n.
   - iMod "H". iSteps.
   - iApply step_fupdN_S_fupd. iSteps.
 Qed.
 
-Lemma wp_adequacy Λ Σ `{inv_Gpre : !invGpreS Σ} e σ :
+Lemma bwp_adequacy Λ Σ `{inv_Gpre : !invGpreS Σ} e σ :
   ( ∀ `{inv_G : !invGS Σ} κs,
     ⊢ |={⊤}=>
-      ∃ state_interp fork_post nt Φ,
+      ∃ state_interp fork_post Φ,
       let iris_G : IrisG Λ Σ := Build_IrisG state_interp fork_post in
-      state_interp nt σ κs ∗
-      WP e {{ Φ }}
+      state_interp 1 σ κs ∗
+      BWP e ∶ 0 {{ Φ }}
   ) →
   safe ([e], σ).
 Proof.
   intros H (es, σ') (n & κs & Hsteps)%silent_steps_nsteps.
-  move: Hsteps. apply: wp_progress => inv_G.
-  iMod H as "(%state_interp & %fork_post & %nt & %Φ & Hσ & H)".
-  iExists state_interp, fork_post, nt, [Φ]. rewrite /wps /=. iSteps.
+  move: Hsteps. apply: bwp_progress => inv_G.
+  iMod H as "(%state_interp & %fork_post & %Φ & Hσ & H)".
+  iExists state_interp, fork_post, [Φ].
+  rewrite /bwps /=. iSteps.
+Qed.
+Lemma wp_adequacy Λ Σ `{inv_Gpre : !invGpreS Σ} e tid σ :
+  (if tid is Some tid then tid = 0 else True) →
+  ( ∀ `{inv_G : !invGS Σ} κs,
+    ⊢ |={⊤}=>
+      ∃ state_interp fork_post Φ,
+      let iris_G : IrisG Λ Σ := Build_IrisG state_interp fork_post in
+      state_interp 1 σ κs ∗
+      WP e ∷ tid {{ Φ }}
+  ) →
+  safe ([e], σ).
+Proof.
+  intros Htid H.
+  apply: bwp_adequacy => inv_G κs.
+  iMod H as "(%state_interp & %fork_post & %Φ & Hσ & H)".
+  iExists state_interp, fork_post, Φ.
+  rewrite wp.wp_unseal.
+  destruct tid; first subst; iSteps.
 Qed.
