theories/zoo/iris/program_logic/ectx_language.v
@@ -12,7 +12,7 @@ Section ectx_language_mixin.
   Context (empty_ectx : ectx).
   Context (comp_ectx : ectx → ectx → ectx).
   Context (fill : ectx → expr → expr).
-  Context (base_step : expr → state → list observation → expr → state → list expr → Prop).
+  Context (base_step : thread_id → expr → state → list observation → expr → state → list expr → Prop).
 
   Record EctxLanguageMixin := {
     mixin_to_of_val v :
@@ -20,8 +20,8 @@ Section ectx_language_mixin.
     mixin_of_to_val e v :
       to_val e = Some v →
       of_val v = e ;
-    mixin_val_base_stuck e1 σ1 κ e2 σ2 es :
-      base_step e1 σ1 κ e2 σ2 es →
+    mixin_val_base_stuck tid e1 σ1 κ e2 σ2 es :
+      base_step tid e1 σ1 κ e2 σ2 es →
       to_val e1 = None ;
 
     mixin_fill_empty e :
@@ -34,15 +34,15 @@ Section ectx_language_mixin.
       is_Some (to_val (fill K e)) →
       is_Some (to_val e) ;
 
-    mixin_step_by_val K' K_redex e1' e1_redex σ1 κ e2 σ2 es :
+    mixin_step_by_val tid K' K_redex e1' e1_redex σ1 κ e2 σ2 es :
       fill K' e1' = fill K_redex e1_redex →
       to_val e1' = None →
-      base_step e1_redex σ1 κ e2 σ2 es →
+      base_step tid e1_redex σ1 κ e2 σ2 es →
         ∃ K'',
         K_redex = comp_ectx K' K'' ;
 
-    mixin_base_ctx_step_val K e σ1 κ e2 σ2 es :
-      base_step (fill K e) σ1 κ e2 σ2 es →
+    mixin_base_ctx_step_val tid K e σ1 κ e2 σ2 es :
+      base_step tid (fill K e) σ1 κ e2 σ2 es →
         is_Some (to_val e) ∨
         K = empty_ectx ;
   }.
@@ -60,7 +60,7 @@ Structure ectx_language := {
   empty_ectx : ectx ;
   comp_ectx : ectx → ectx → ectx ;
   fill : ectx → expr → expr ;
-  base_step : expr → state → list observation → expr → state → list expr → Prop ;
+  base_step : thread_id → expr → state → list observation → expr → state → list expr → Prop ;
 
   ectx_language_mixin : EctxLanguageMixin of_val to_val empty_ectx comp_ectx fill base_step ;
 }.
@@ -74,7 +74,7 @@ Bind Scope val_scope with val.
 #[global] Arguments empty_ectx {_} : assert.
 #[global] Arguments comp_ectx {_} _ _ : assert.
 #[global] Arguments fill {_} _ _ : assert.
-#[global] Arguments base_step {_} _ _ _ _ _ _ : assert.
+#[global] Arguments base_step {_} _ _ _ _ _ _ _ : assert.
 
 Section ectx_language.
   Context {Λ : ectx_language}.
@@ -85,55 +85,55 @@ Section ectx_language.
   Implicit Types K : ectx Λ.
   Implicit Types κ : list (observation Λ).
 
-  Definition base_reducible e σ :=
+  Definition base_reducible tid e σ :=
     ∃ κ e' σ' es,
-    base_step e σ κ e' σ' es.
-  Definition base_reducible_no_obs e σ :=
+    base_step tid e σ κ e' σ' es.
+  Definition base_reducible_no_obs tid e σ :=
     ∃ e' σ' es,
-    base_step e σ [] e' σ' es.
-  Definition base_irreducible e σ :=
+    base_step tid e σ [] e' σ' es.
+  Definition base_irreducible tid e σ :=
     ∀ κ e' σ' es,
-    ¬ base_step e σ κ e' σ' es.
-  Definition base_stuck e σ :=
+    ¬ base_step tid e σ κ e' σ' es.
+  Definition base_stuck tid e σ :=
     to_val e = None ∧
-    base_irreducible e σ.
+    base_irreducible tid e σ.
 
   Definition sub_redexes_are_values e :=
     ∀ K e', e = fill K e' →
     to_val e' = None →
     K = empty_ectx.
 
-  Inductive prim_step e1 σ1 κ e2 σ2 es : Prop :=
+  Inductive prim_step tid e1 σ1 κ e2 σ2 es : Prop :=
     | base_step_fill_prim_step' K e1' e2' :
         e1 = fill K e1' →
         e2 = fill K e2' →
-        base_step e1' σ1 κ e2' σ2 es →
-        prim_step e1 σ1 κ e2 σ2 es.
+        base_step tid e1' σ1 κ e2' σ2 es →
+        prim_step tid e1 σ1 κ e2 σ2 es.
 
   Definition base_atomic e :=
-    ∀ σ κ e' σ' es,
-    base_step e σ κ e' σ' es →
+    ∀ tid σ κ e' σ' es,
+    base_step tid e σ κ e' σ' es →
     is_Some (to_val e').
 
   Record pure_base_step e1 e2 := {
-    pure_base_step_safe σ1 :
-      base_reducible_no_obs e1 σ1 ;
-    pure_base_step_det σ1 κ e2' σ2 es :
-      base_step e1 σ1 κ e2' σ2 es →
+    pure_base_step_safe tid σ1 :
+      base_reducible_no_obs tid e1 σ1 ;
+    pure_base_step_det tid σ1 κ e2' σ2 es :
+      base_step tid e1 σ1 κ e2' σ2 es →
         κ = [] ∧
         σ2 = σ1 ∧
         e2' = e2 ∧
         es = [] ;
   }.
 
-  Lemma base_step_not_val e1 σ1 κ e2 σ2 es :
-    base_step e1 σ1 κ e2 σ2 es →
+  Lemma base_step_not_val tid e1 σ1 κ e2 σ2 es :
+    base_step tid e1 σ1 κ e2 σ2 es →
     to_val e1 = None.
   Proof.
     apply ectx_language_mixin.
   Qed.
-  Lemma base_reducible_not_val e σ :
-    base_reducible e σ →
+  Lemma base_reducible_not_val tid e σ :
+    base_reducible tid e σ →
     to_val e = None.
   Proof.
     intros (κ & e' & σ' & es & He%base_step_not_val). done.
@@ -161,27 +161,27 @@ Section ectx_language.
     apply ectx_language_mixin.
   Qed.
 
-  Lemma step_by_val K' K_redex e1' e1_redex σ1 κ e2 σ2 es :
+  Lemma step_by_val tid K' K_redex e1' e1_redex σ1 κ e2 σ2 es :
     fill K' e1' = fill K_redex e1_redex →
     to_val e1' = None →
-    base_step e1_redex σ1 κ e2 σ2 es →
+    base_step tid e1_redex σ1 κ e2 σ2 es →
       ∃ K'',
       K_redex = comp_ectx K' K''.
   Proof.
     apply ectx_language_mixin.
   Qed.
 
-  Lemma base_ctx_step_val K e σ1 κ e2 σ2 es :
-    base_step (fill K e) σ1 κ e2 σ2 es →
+  Lemma base_ctx_step_val tid K e σ1 κ e2 σ2 es :
+    base_step tid (fill K e) σ1 κ e2 σ2 es →
       is_Some (to_val e) ∨
       K = empty_ectx.
   Proof.
     apply ectx_language_mixin.
   Qed.
 
-  Lemma base_step_fill_prim_step K e1 σ1 κ e2 σ2 es :
-    base_step e1 σ1 κ e2 σ2 es →
-    prim_step (fill K e1) σ1 κ (fill K e2) σ2 es.
+  Lemma base_step_fill_prim_step tid K e1 σ1 κ e2 σ2 es :
+    base_step tid e1 σ1 κ e2 σ2 es →
+    prim_step tid (fill K e1) σ1 κ (fill K e2) σ2 es.
   Proof.
     eauto using prim_step.
   Qed.
@@ -192,7 +192,7 @@ Section ectx_language.
     split.
     - apply ectx_language_mixin.
     - apply ectx_language_mixin.
-    - intros ? ? ? ? ? ? [? ? ? -> -> ?%base_step_not_val].
+    - intros ? ? ? ? ? ? ? [? ? ? -> -> ?%base_step_not_val].
       apply eq_None_not_Some. intros ?%fill_val%eq_None_not_Some; done.
   Qed.
   Canonical ectx_lang :=
@@ -205,128 +205,131 @@ Section ectx_language.
     rewrite !eq_None_not_Some. eauto using fill_val.
   Qed.
 
-  Lemma base_reducible_no_obs_base_reducible e σ :
-    base_reducible_no_obs e σ →
-    base_reducible e σ.
+  Lemma base_reducible_no_obs_base_reducible tid e σ :
+    base_reducible_no_obs tid e σ →
+    base_reducible tid e σ.
   Proof.
     intros (? & ? & ? & ?). eexists. eauto.
   Qed.
-  Lemma not_base_reducible e σ :
-    ¬ base_reducible e σ ↔
-    base_irreducible e σ.
+  Lemma not_base_reducible tid e σ :
+    ¬ base_reducible tid e σ ↔
+    base_irreducible tid e σ.
   Proof.
     rewrite /base_reducible /base_irreducible. naive_solver.
   Qed.
 
-  Lemma base_redex_unique K K' e e' σ :
+  Lemma base_redex_unique tid K e K' e' σ :
     fill K e = fill K' e' →
-    base_reducible e σ →
-    base_reducible e' σ →
+    base_reducible tid e σ →
+    base_reducible tid e' σ →
       K = comp_ectx K' empty_ectx ∧
       e = e'.
   Proof.
     intros Heq (κ & e2 & σ2 & es & Hred) (κ' & e2' & σ2' & es' & Hred').
-    edestruct (step_by_val K' K e' e) as [K'' HK]; [eauto using base_step_not_val.. |].
+    edestruct (step_by_val tid K' K e' e) as [K'' HK]; [eauto using base_step_not_val.. |].
     subst K. move: Heq. rewrite -fill_comp. intros <-%(inj (fill _)).
-    destruct (base_ctx_step_val _ _ _ _ _ _ _ Hred') as [[]%not_eq_None_Some | HK''].
+    odestruct base_ctx_step_val as [[]%not_eq_None_Some | HK''].
+    { done. }
     { eapply base_step_not_val. done. }
     subst K''. rewrite fill_empty //.
   Qed.
 
-  Lemma base_step_prim_step e1 σ1 κ e2 σ2 es :
-    base_step e1 σ1 κ e2 σ2 es →
-    prim_step e1 σ1 κ e2 σ2 es.
+  Lemma base_step_prim_step tid e1 σ1 κ e2 σ2 es :
+    base_step tid e1 σ1 κ e2 σ2 es →
+    prim_step tid e1 σ1 κ e2 σ2 es.
   Proof.
     apply base_step_fill_prim_step' with empty_ectx.
     all: rewrite ?fill_empty //.
   Qed.
 
-  Lemma base_step_not_stuck e σ κ e' σ' es :
-    base_step e σ κ e' σ' es →
-    not_stuck e σ.
+  Lemma base_step_not_stuck tid e σ κ e' σ' es :
+    base_step tid e σ κ e' σ' es →
+    not_stuck tid e σ.
   Proof.
     rewrite /not_stuck /reducible /=.
     eauto 10 using base_step_prim_step.
   Qed.
 
-  Lemma fill_prim_step K e1 σ1 κ e2 σ2 es :
-    prim_step e1 σ1 κ e2 σ2 es →
-    prim_step (fill K e1) σ1 κ (fill K e2) σ2 es.
+  Lemma fill_prim_step tid K e1 σ1 κ e2 σ2 es :
+    prim_step tid e1 σ1 κ e2 σ2 es →
+    prim_step tid (fill K e1) σ1 κ (fill K e2) σ2 es.
   Proof.
     destruct 1 as [K' e1' e2' -> ->].
     rewrite !fill_comp. econstructor; done.
   Qed.
-  Lemma fill_reducible K e σ :
-    reducible e σ →
-    reducible (fill K e) σ.
+  Lemma fill_reducible tid K e σ :
+    reducible tid e σ →
+    reducible tid (fill K e) σ.
   Proof.
     intros (κ & e' & σ' & es & ?). exists κ, (fill K e'), σ', es.
     apply fill_prim_step. done.
   Qed.
-  Lemma fill_reducible_no_obs K e σ :
-    reducible_no_obs e σ →
-    reducible_no_obs (fill K e) σ.
+  Lemma fill_reducible_no_obs tid K e σ :
+    reducible_no_obs tid e σ →
+    reducible_no_obs tid (fill K e) σ.
   Proof.
     intros (e' & σ' & es & ?). exists (fill K e'), σ', es.
     apply fill_prim_step. done.
   Qed.
-  Lemma base_reducible_reducible e σ :
-    base_reducible e σ →
-    reducible e σ.
+  Lemma base_reducible_reducible tid e σ :
+    base_reducible tid e σ →
+    reducible tid e σ.
   Proof.
-    intros (κ & e' & σ' & es & ?). eexists κ, e', σ', es.
+    intros (κ & e' & σ' & es & ?).
+    exists κ, e', σ', es.
     apply base_step_prim_step. done.
   Qed.
-  Lemma base_reducible_prim_fill_reducible e K σ :
-    base_reducible e σ →
-    reducible (fill K e) σ.
+  Lemma base_reducible_prim_fill_reducible tid e K σ :
+    base_reducible tid e σ →
+    reducible tid (fill K e) σ.
   Proof.
     intro.
     apply fill_reducible, base_reducible_reducible. done.
   Qed.
-  Lemma base_reducible_no_obs_reducible e σ :
-    base_reducible_no_obs e σ →
-    reducible_no_obs e σ.
+  Lemma base_reducible_no_obs_reducible tid e σ :
+    base_reducible_no_obs tid e σ →
+    reducible_no_obs tid e σ.
   Proof.
-    intros (e' & σ' & es & ?). eexists e', σ', es.
+    intros (e' & σ' & es & ?).
+    exists e', σ', es.
     apply base_step_prim_step. done.
   Qed.
-  Lemma irreducible_base_irreducible e σ :
-    irreducible e σ →
-    base_irreducible e σ.
+  Lemma irreducible_base_irreducible tid e σ :
+    irreducible tid e σ →
+    base_irreducible tid e σ.
   Proof.
     rewrite -not_reducible -not_base_reducible.
     auto using base_reducible_reducible.
   Qed.
-  Lemma base_reducible_no_obs_fill_reducible e K σ :
-    base_reducible_no_obs e σ →
-    reducible_no_obs (fill K e) σ.
+  Lemma base_reducible_no_obs_fill_reducible tid e K σ :
+    base_reducible_no_obs tid e σ →
+    reducible_no_obs tid (fill K e) σ.
   Proof.
     intro.
     apply fill_reducible_no_obs, base_reducible_no_obs_reducible. done.
   Qed.
 
-  Lemma reducible_base_reducible e σ :
-    reducible e σ →
+  Lemma reducible_base_reducible tid e σ :
+    reducible tid e σ →
     sub_redexes_are_values e →
-    base_reducible e σ.
+    base_reducible tid e σ.
   Proof.
     intros (κ & e' & σ' & es & [K e1' e2' -> -> Hstep]) ?.
     assert (K = empty_ectx) as -> by eauto 10 using base_step_not_val.
     rewrite fill_empty /base_reducible. eauto 10.
   Qed.
-  Lemma base_irreducible_irreducible e σ :
-    base_irreducible e σ →
+  Lemma base_irreducible_irreducible tid e σ :
+    base_irreducible tid e σ →
     sub_redexes_are_values e →
-    irreducible e σ.
+    irreducible tid e σ.
   Proof.
     rewrite -not_reducible -not_base_reducible.
     auto using reducible_base_reducible.
   Qed.
-  Lemma base_stuck_stuck e σ :
-    base_stuck e σ →
+  Lemma base_stuck_stuck tid e σ :
+    base_stuck tid e σ →
     sub_redexes_are_values e →
-    stuck e σ.
+    stuck tid e σ.
   Proof.
     intros [] ?.
     split; first done.
@@ -338,34 +341,33 @@ Section ectx_language.
     sub_redexes_are_values e →
     Atomic e.
   Proof.
-    intros Hatomic_step Hatomic_fill σ κ e' σ' es [K e1' e2' -> -> Hstep].
+    intros Hatomic_step Hatomic_fill tid σ κ e' σ' es [K e1' e2' -> -> Hstep].
     assert (K = empty_ectx) as -> by eauto 10 using base_step_not_val.
     rewrite fill_empty. eapply Hatomic_step. rewrite fill_empty //.
   Qed.
 
-  Lemma base_reducible_fill_prim_step K e1 σ1 κ e2 σ2 es :
-    base_reducible e1 σ1 →
-    prim_step (fill K e1) σ1 κ e2 σ2 es →
+  Lemma base_reducible_fill_prim_step tid K e1 σ1 κ e2 σ2 es :
+    base_reducible tid e1 σ1 →
+    prim_step tid (fill K e1) σ1 κ e2 σ2 es →
       ∃ e2',
       e2 = fill K e2' ∧
-      base_step e1 σ1 κ e2' σ2 es.
+      base_step tid e1 σ1 κ e2' σ2 es.
   Proof.
     intros (κ' & e2'' & σ2'' & es'' & HhstepK) [K' e1' e2' HKe1 -> Hstep].
-    edestruct (step_by_val K) as [K'' ?]; eauto using base_step_not_val; simplify_eq/=.
+    edestruct (step_by_val tid K) as [K'' ?]; eauto using base_step_not_val; simplify_eq/=.
     rewrite -fill_comp in HKe1; simplify_eq.
     exists (fill K'' e2'). rewrite fill_comp; split; first done.
     apply base_ctx_step_val in HhstepK as [[v ?] | ?]; simplify_eq.
     { apply base_step_not_val in Hstep. simplify_eq. }
     rewrite !fill_empty //.
   Qed.
-
-  Lemma base_reducible_prim_step e1 σ1 κ e2 σ2 es :
-    base_reducible e1 σ1 →
-    prim_step e1 σ1 κ e2 σ2 es →
-    base_step e1 σ1 κ e2 σ2 es.
+  Lemma base_reducible_prim_step tid e1 σ1 κ e2 σ2 es :
+    base_reducible tid e1 σ1 →
+    prim_step tid e1 σ1 κ e2 σ2 es →
+    base_step tid e1 σ1 κ e2 σ2 es.
   Proof.
     intros.
-    edestruct (base_reducible_fill_prim_step empty_ectx) as (? & ? & ?).
+    edestruct (base_reducible_fill_prim_step tid empty_ectx) as (? & ? & ?).
     all: rewrite ?fill_empty; eauto.
     simplify. rewrite fill_empty //.
   Qed.
@@ -375,10 +377,12 @@ Section ectx_language.
     pure_step e1 e2.
   Proof.
     intros [Hsafe Hdet]. split.
-    - intros σ. destruct (Hsafe σ) as (e2' & σ2 & es & ?).
-      eexists e2', σ2, es. apply base_step_prim_step. done.
-    - intros σ1 κ e2' σ2 es ?%base_reducible_prim_step.
-      all: auto using base_reducible_no_obs_base_reducible.
+    - intros tid σ.
+      destruct (Hsafe tid σ) as (e2' & σ2 & es & ?).
+      exists e2', σ2, es.
+      apply base_step_prim_step. done.
+    - intros tid σ1 κ e2' σ2 es ?%base_reducible_prim_step.
+      all: eauto using base_reducible_no_obs_base_reducible.
   Qed.
 
   #[global] Instance ectx_lang_ctx K :
@@ -386,12 +390,13 @@ Section ectx_language.
   Proof.
     split; simpl.
     - auto using fill_not_val.
-    - intros ? ? ? ? ? ? [K' e1' e2' Heq1 Heq2 Hstep].
-      exists (comp_ectx K K') e1' e2'; rewrite ?Heq1 ?Heq2 ?fill_comp //.
-    - intros e1 σ1 κ e2 σ2 es Hnval [K'' e1'' e2'' Heq1 -> Hstep].
-      destruct (step_by_val K K'' e1 e1'' σ1 κ e2'' σ2 es) as [K' ->]; auto.
-      rewrite -fill_comp in Heq1; apply (inj (fill _)) in Heq1.
-      exists (fill K' e2''); rewrite -fill_comp; split; auto.
+    - intros ? ? ? ? ? ? ? [K' e1' e2' Heq1 Heq2 Hstep].
+      exists (comp_ectx K K') e1' e2'.
+      all: rewrite ?Heq1 ?Heq2 ?fill_comp //.
+    - intros tid e1 σ1 κ e2 σ2 es Hnval [K'' e1'' e2'' Heq1 -> Hstep].
+      destruct (step_by_val tid K K'' e1 e1'' σ1 κ e2'' σ2 es) as [K' ->]; try done.
+      rewrite -fill_comp in Heq1. apply (inj (fill _)) in Heq1.
+      exists (fill K' e2''). rewrite -fill_comp. split; first done.
       eauto using prim_step.
   Qed.
 
@@ -426,7 +431,7 @@ Section ectx_language.
   Qed.
 End ectx_language.
 
-#[global] Arguments base_step_fill_prim_step' {_ _ _ _ _ _ _}.
+#[global] Arguments base_step_fill_prim_step' {_ _ _ _ _ _ _ _}.
 
 #[global] Arguments ectx_lang : clear implicits.
 Coercion ectx_lang : ectx_language >-> language.
