theories/zoo/iris/program_logic/wp.v
@@ -1,165 +1,118 @@
-From iris.base_logic Require Export
-  lib.fancy_updates.
-
 From zoo Require Import
   prelude.
 From zoo.iris Require Import
   diaframe.
 From zoo.iris.program_logic Require Export
-  language.
+  bwp.
 From zoo Require Import
   options.
-
-Class IrisG Λ Σ := {
-  #[global] iris_G_inv_G :: invGS Σ ;
-  state_interp : nat → state Λ → list (observation Λ) → iProp Σ ;
-  fork_post : val Λ → iProp Σ ;
-}.
-#[global] Arguments Build_IrisG {_ _ _} _ _ : assert.
-#[global] Opaque iris_G_inv_G.
 
 Section iris_G.
   Context `{iris_G : !IrisG Λ Σ}.
 
-  Definition wp_pre (wp : expr Λ -d> coPset -d> (val Λ -d> iPropO Σ) -d> iPropO Σ)
-  : expr Λ -d> coPset -d> (val Λ -d> iPropO Σ) -d> iPropO Σ
-  :=
-    λ e E Φ,
-      match to_val e with
-      | Some v =>
-          |={E}=> Φ v
-      | None =>
-          ∀ nt σ κ κs,
-          state_interp nt σ (κ ++ κs) -∗
-            |={E, ∅}=>
-            ⌜reducible e σ⌝ ∗
-              ∀ e' σ' es,
-              ⌜prim_step e σ κ e' σ' es⌝ -∗
-              £ 1 -∗
-                |={∅}=> ▷ |={∅, E}=>
-                state_interp (nt + length es) σ' κs ∗
-                wp e' E Φ ∗
-                [∗ list] i ↦ e ∈ es,
-                  wp e ⊤ fork_post
-      end%I.
-  #[global] Arguments wp_pre _ e%_E E Φ%_I : rename.
-
-  #[local] Instance wp_pre_contractive :
-    Contractive wp_pre.
-  Proof.
-    rewrite /wp_pre /= => n wp1 wp2 Hwp e E Φ.
-    repeat (apply Hwp || f_contractive || f_equiv).
-  Qed.
-
-  #[local] Definition wp_def :=
-    fixpoint wp_pre.
-  #[global] Arguments wp_def e%_E E Φ%_I : rename.
+  #[local] Definition wp_def e tid E Φ :=
+    match tid with
+    | None =>
+        ∀ tid, BWP e ∶ tid @ E {{ Φ }}
+    | Some tid =>
+        BWP e ∶ tid @ E {{ Φ }}
+    end%I.
+  #[global] Arguments wp_def _ _%_E _ _%_I : assert.
 End iris_G.
 
 #[local] Definition wp_aux : seal (@wp_def).
   Proof. by eexists. Qed.
 Definition wp :=
   wp_aux.(unseal).
-#[global] Arguments wp {_ _ _} e%_E E Φ%_I : rename.
+#[global] Arguments wp {_ _ _} _ _%_E _ _%_I : assert.
 #[local] Lemma wp_unseal `{iris_G : !IrisG Λ Σ} :
   wp = @wp_def Λ Σ _.
 Proof.
   rewrite -wp_aux.(seal_eq) //.
 Qed.
 
-Notation "'WP' e @ E {{ Φ } }" := (
-  wp e%E E Φ
-)(at level 20,
-  e, Φ at level 200,
-  only parsing
-) : bi_scope.
-Notation "'WP' e {{ Φ } }" := (
-  wp e%E ⊤ Φ
-)(at level 20,
-  e, Φ at level 200,
-  only parsing
-) : bi_scope.
+#[local] Ltac wp_unseal :=
+  rewrite wp_unseal /wp_def;
+  select (option thread_id) (fun tid => destruct tid).
 
-Notation "'WP' e @ E {{ v , Q } }" := (
-  wp e%E E (λ v, Q)
+Declare Custom Entry wp_thread_id.
+Notation "" := (
+  None
+)(in custom wp_thread_id
+).
+Notation "∶ tid" := (
+  Some tid
+)(in custom wp_thread_id at level 200,
+  tid constr,
+  format "'/  ' ∶  tid "
+).
+Notation "∷ tid" :=
+  tid
+( in custom wp_thread_id at level 200,
+  tid constr,
+  format "'/  ' ∷  tid "
+).
+
+Notation "'WP' e tid E {{ Φ } }" := (
+  wp e%E tid E Φ%I
 )(at level 20,
-  e, Q at level 200,
+  e at level 200,
+  tid custom wp_thread_id at level 200,
+  E custom wp_mask at level 200,
+  Φ at level 200,
+  format "'[hv' WP  '/  ' '[' e ']'  tid E '/' {{  '[' Φ ']'  '/' } } ']'"
+) : bi_scope.
+Notation "'WP' e tid E {{ v , Q } }" := (
+  wp e%E tid E (λ v, Q%I)
+)(at level 20,
+  e at level 200,
+  tid custom wp_thread_id at level 200,
+  E custom wp_mask at level 200,
+  Q at level 200,
   v at level 200 as pattern,
-  format "'[hv' 'WP'  e  '/' @  E  '/' {{  '[' v ,  '/' Q  ']' } } ']'"
-) : bi_scope.
-Notation "'WP' e {{ v , Q } }" := (
-  wp e%E ⊤ (λ v, Q)
-)(at level 20,
-  e, Q at level 200,
-  v at level 200 as pattern,
-  format "'[hv' 'WP'  e  '/' {{  '[' v ,  '/' Q  ']' } } ']'"
+  format "'[hv' WP  '/  ' '[' e ']'  tid E '/' {{  '[' v ,  '/' Q ']'  '/' } } ']'"
 ) : bi_scope.
 
-Notation "'{{{' P } } } e @ E {{{ x .. y , 'RET' pat ; Q } } }" :=
+Notation "'{{{' P } } } e tid E {{{ x1 .. xn , 'RET' v ; Q } } }" :=
   ( □ ∀ Φ,
       P -∗
-      ▷ (∀ x, .. (∀ y, Q -∗ Φ pat%V) ..) -∗
-      WP e @ E {{ Φ }}
+      ▷ (∀ x1, .. (∀ xn, Q -∗ Φ v%V) ..) -∗
+      wp e%E tid E Φ
   )%I
 ( at level 20,
-  x closed binder,
-  y closed binder,
-  format "'[hv' {{{  '[' P  ']' } } }  '/  ' e  '/' @  E  '/' {{{  '[' x  ..  y ,  RET  pat ;  '/' Q  ']' } } } ']'"
+  P at level 200,
+  e at level 200,
+  tid custom wp_thread_id at level 200,
+  E custom wp_mask at level 200,
+  x1 closed binder,
+  xn closed binder,
+  format "'[hv' {{{  '/  ' '[' P ']'  '/' } } }  '/  ' '[' e ']'  tid E '/' {{{  x1  ..  xn ,  '/  ' RET  v ;  '/  ' '[' Q ']'  '/' } } } ']'"
 ) : bi_scope.
-Notation "'{{{' P } } } e {{{ x .. y , 'RET' pat ; Q } } }" :=
+Notation "'{{{' P } } } e tid E {{{ 'RET' v ; Q } } }" :=
   ( □ ∀ Φ,
       P -∗
-      ▷ (∀ x, .. (∀ y, Q -∗ Φ pat%V) ..) -∗
-      WP e {{ Φ }}
+      ▷ (Q -∗ Φ v%V) -∗
+      wp e%E tid E Φ
   )%I
 ( at level 20,
-  x closed binder,
-  y closed binder,
-  format "'[hv' {{{  '[' P  ']' } } }  '/  ' e  '/' {{{  '[' x  ..  y ,  RET  pat ;  '/' Q  ']' } } } ']'"
-) : bi_scope.
-
-Notation "'{{{' P } } } e @ E {{{ 'RET' pat ; Q } } }" :=
-  ( □ ∀ Φ,
-      P -∗
-      ▷ (Q -∗ Φ pat%V) -∗
-      WP e @ E {{ Φ }}
-  )%I
-( at level 20,
-  format "'[hv' {{{  '[' P  ']' } } }  '/  ' e  '/' @  E  '/' {{{  '[' RET  pat ;  '/' Q  ']' } } } ']'"
-) : bi_scope.
-Notation "'{{{' P } } } e {{{ 'RET' pat ; Q } } }" :=
-  ( □ ∀ Φ,
-      P -∗
-      ▷ (Q -∗ Φ pat%V) -∗
-      WP e {{ Φ }}
-  )%I
-( at level 20,
-  format "'[hv' {{{  '[' P  ']' } } }  '/  ' e  '/' {{{  '[' RET  pat ;  '/' Q  ']' } } } ']'"
+  P at level 200,
+  e at level 200,
+  tid custom wp_thread_id at level 200,
+  E custom wp_mask at level 200,
+  format "'[hv' {{{  '/  ' '[' P ']'  '/' } } }  '/  ' '[' e ']'  tid E '/' {{{  '/  ' RET  v ;  '/  ' '[' Q ']'  '/' } } } ']'"
 ) : bi_scope.
 
-Notation "'{{{' P } } } e @ E {{{ x .. y , 'RET' pat ; Q } } }" := (
+Notation "'{{{' P } } } e tid E {{{ x1 .. xn , 'RET' v ; Q } } }" := (
   ∀ Φ,
-  P -∗
-  ▷ (∀ x, .. (∀ y, Q -∗ Φ pat%V) ..) -∗
-  WP e @ E {{ Φ }}
+  P%I -∗
+  ▷ (∀ x1, .. (∀ xn, Q%I -∗ Φ v%V) ..) -∗
+  wp e%E tid E Φ%I
 ) : stdpp_scope.
-Notation "'{{{' P } } } e {{{ x .. y , 'RET' pat ; Q } } }" := (
+Notation "'{{{' P } } } e tid E {{{ 'RET' v ; Q } } }" := (
   ∀ Φ,
-  P -∗
-  ▷ (∀ x, .. (∀ y, Q -∗ Φ pat%V) ..) -∗
-  WP e {{ Φ }}
-) : stdpp_scope.
-Notation "'{{{' P } } } e @ E {{{ 'RET' pat ; Q } } }" := (
-  ∀ Φ,
-  P -∗
-  ▷ (Q -∗ Φ pat%V) -∗
-  WP e @ E {{ Φ }}
-) : stdpp_scope.
-Notation "'{{{' P } } } e {{{ 'RET' pat ; Q } } }" := (
-  ∀ Φ,
-  P -∗
-  ▷ (Q -∗ Φ pat%V) -∗
-  WP e {{ Φ }}
+  P%I -∗
+  ▷ (Q%I -∗ Φ v%V) -∗
+  wp e%E tid E Φ%I
 ) : stdpp_scope.
 
 Section iris_G.
@@ -170,314 +123,269 @@ Section iris_G.
   Implicit Types P R : iProp Σ.
   Implicit Types Φ : val Λ → iProp Σ.
 
-  Lemma wp_unfold e E Φ :
-    WP e @ E {{ Φ }} ⊣⊢
-    wp_pre wp e E Φ.
+  #[global] Instance wp_ne n e tid E :
+    Proper (pointwise_relation _ (≡{n}≡) ==> (≡{n}≡)) (wp e tid E).
   Proof.
-    rewrite wp_unseal. apply (fixpoint_unfold wp_pre).
+    rewrite wp_unseal. solve_proper.
   Qed.
-
-  #[global] Instance wp_ne n e E :
-    Proper (pointwise_relation _ (≡{n}≡) ==> (≡{n}≡)) (wp e E).
+  #[global] Instance wp_proper e tid E :
+    Proper (pointwise_relation _ (≡) ==> (≡)) (wp e tid E).
   Proof.
-    move: e. induction (lt_wf n) as [n _ IH] => e Φ1 Φ2 HΦ.
-    rewrite !wp_unfold /wp_pre /=.
-    do 25 (f_contractive || f_equiv).
-    apply IH; first done.
-    f_equiv.
-    eapply dist_le; [apply HΦ | lia].
+    rewrite wp_unseal. solve_proper.
   Qed.
-  #[global] Instance wp_proper e E :
-    Proper (pointwise_relation _ (≡) ==> (≡)) (wp e E).
-  Proof.
-    intros Φ1 Φ2 HΦ.
-    apply equiv_dist => n. apply wp_ne => v. apply equiv_dist. done.
-  Qed.
-  #[global] Instance wp_contractive n e E :
+  #[global] Instance wp_contractive n e tid E :
     TCEq (to_val e) None →
-    Proper (pointwise_relation _ (dist_later n) ==> (≡{n}≡)) (wp e E).
+    Proper (pointwise_relation _ (dist_later n) ==> (≡{n}≡)) (wp e tid E).
   Proof.
-    intros He Φ1 Φ2 HΦ.
-    rewrite !wp_unfold /wp_pre He /=.
-    repeat (f_contractive || f_equiv).
+    wp_unseal.
+    - apply bwp_contractive.
+    - intros He Φ1 Φ2 HΦ.
+      f_equiv => tid.
+      apply bwp_contractive; done.
   Qed.
 
-  Lemma wp_value_fupd' v E Φ :
-    WP of_val v @ E {{ Φ }} ⊣⊢
+  Lemma wp_thread_id_mono e tid E Φ :
+    WP e @ E {{ Φ }} ⊢
+    WP e ∷ tid @ E {{ Φ }}.
+  Proof.
+    wp_unseal.
+    all: iSteps.
+  Qed.
+
+  Lemma wp_bwp e tid E Φ :
+    WP e @ E {{ Φ }} ⊢
+    BWP e ∶ tid @ E {{ Φ }}.
+  Proof.
+    rewrite wp_unseal. iSteps.
+  Qed.
+  Lemma bwp_wp e tid E Φ :
+    (∀ tid, BWP e ∶ tid @ E {{ Φ }}) ⊢
+    WP e ∷ tid @ E {{ Φ }}.
+  Proof.
+    rewrite -wp_thread_id_mono wp_unseal //.
+  Qed.
+
+  Lemma wp_value_fupd' v tid E Φ :
+    WP of_val v ∷ tid @ E {{ Φ }} ⊣⊢
     |={E}=> Φ v.
   Proof.
-    rewrite wp_unfold /wp_pre to_of_val //.
+    wp_unseal.
+    - apply bwp_value_fupd'.
+    - iSplit.
+      + iIntros "H".
+        iSpecialize ("H" $! 0).
+        rewrite bwp_value_fupd' //.
+      + iIntros "H %tid".
+        rewrite bwp_value_fupd' //.
   Qed.
-  Lemma wp_value_fupd e v E Φ :
+  Lemma wp_value_fupd e v tid E Φ :
     AsVal e v →
-    WP e @ E {{ Φ }} ⊣⊢
+    WP e ∷ tid @ E {{ Φ }} ⊣⊢
     |={E}=> Φ v.
   Proof.
     rewrite -wp_value_fupd' => <- //.
   Qed.
-  Lemma wp_value' v E Φ :
+  Lemma wp_value' v tid E Φ :
     Φ v ⊢
-    WP (of_val v) @ E {{ Φ }}.
+    WP of_val v ∷ tid @ E {{ Φ }}.
   Proof.
     rewrite wp_value_fupd'. auto.
   Qed.
-  Lemma wp_value e v E Φ :
+  Lemma wp_value e v tid E Φ :
     AsVal e v →
     Φ v ⊢
-    WP e @ E {{ Φ }}.
+    WP e ∷ tid @ E {{ Φ }}.
   Proof.
     rewrite wp_value' => <- //.
   Qed.
 
-  Lemma wp_strong_mono e E1 Φ1 E2 Φ2 :
+  Lemma wp_strong_mono e tid E1 Φ1 E2 Φ2 :
     E1 ⊆ E2 →
-    WP e @ E1 {{ Φ1 }} -∗
+    WP e ∷ tid @ E1 {{ Φ1 }} -∗
     (∀ v, Φ1 v ={E2}=∗ Φ2 v) -∗
-    WP e @ E2 {{ Φ2 }}.
+    WP e ∷ tid @ E2 {{ Φ2 }}.
   Proof.
-    iIntros "%HE H HΦ".
-    iLöb as "HLöb" forall (e).
-    rewrite !wp_unfold /wp_pre /=.
-    destruct (to_val e) as [v |] eqn:He.
-    - iApply ("HΦ" with "[> H]").
-      iSteps.
-    - iIntros "%nt %σ1 %κ %κs Hσ".
-      iMod (fupd_mask_subseteq E1) as "Hclose"; first done.
-      iMod ("H" with "Hσ") as "(%Hreducible & H)".
-      iModIntro. iStep. iIntros "%e2 %σ2 %es %Hstep H£".
-      iMod ("H" with "[//] H£") as "H".
-      do 2 iModIntro.
-      iMod "H" as "($ & H & Hes)".
-      iMod "Hclose" as "_".
-      iSplitR "Hes"; iSteps.
+    wp_unseal.
+    - apply bwp_strong_mono.
+    - iIntros "%HE H HΦ %tid".
+      iApply (bwp_strong_mono with "H HΦ"); first done.
   Qed.
-  Lemma wp_mono e E Φ1 Φ2 :
+  Lemma wp_mono e tid E Φ1 Φ2 :
     (∀ v, Φ1 v ⊢ Φ2 v) →
-    WP e @ E {{ Φ1 }} ⊢
-    WP e @ E {{ Φ2 }}.
+    WP e ∷ tid @ E {{ Φ1 }} ⊢
+    WP e ∷ tid @ E {{ Φ2 }}.
   Proof.
     iIntros "%HΦ H".
     iApply (wp_strong_mono with "H"); first done. iIntros "%v HΦ".
     iApply (HΦ with "HΦ").
   Qed.
-  Lemma wp_mask_mono e E1 E2 Φ :
-    E1 ⊆ E2 →
-    WP e @ E1 {{ Φ }} ⊢
-    WP e @ E2 {{ Φ }}.
-  Proof.
-    iIntros "%HE H".
-    iApply (wp_strong_mono with "H"); first done.
-    iSteps.
-  Qed.
-  #[global] Instance wp_mono' e E :
-    Proper (pointwise_relation _ (⊢) ==> (⊢)) (wp e E).
+  #[global] Instance wp_mono' e tid E :
+    Proper (pointwise_relation _ (⊢) ==> (⊢)) (wp e tid E).
   Proof.
     intros Φ1 Φ2 HΦ.
     apply wp_mono. done.
   Qed.
-  #[global] Instance wp_flip_mono' e E :
-    Proper (pointwise_relation _ (flip (⊢)) ==> (flip (⊢))) (wp e E).
+  #[global] Instance wp_flip_mono' e tid E :
+    Proper (pointwise_relation _ (flip (⊢)) ==> (flip (⊢))) (wp e tid E).
   Proof.
     solve_proper.
   Qed.
 
-  Lemma fupd_wp e E Φ :
-    (|={E}=> WP e @ E {{ Φ }}) ⊢
-    WP e @ E {{ Φ }}.
+  Lemma fupd_wp e tid E Φ :
+    (|={E}=> WP e ∷ tid @ E {{ Φ }}) ⊢
+    WP e ∷ tid @ E {{ Φ }}.
   Proof.
-    iIntros "H".
-    rewrite wp_unfold /wp_pre.
-    destruct (to_val e) as [v |] eqn:He; first iSteps.
-    iIntros "%nt %σ1 %κ %κs Hσ".
-    iMod "H".
-    iApply ("H" with "Hσ").
+    wp_unseal.
+    - apply fupd_bwp.
+    - iIntros "H %tid".
+      iSpecialize ("H" $! tid).
+      iApply (fupd_bwp with "H").
   Qed.
-  Lemma wp_fupd e E Φ :
-    WP e @ E {{ v, |={E}=> Φ v }} ⊢
-    WP e @ E {{ Φ }}.
+  Lemma wp_fupd e tid E Φ :
+    WP e ∷ tid @ E {{ v, |={E}=> Φ v }} ⊢
+    WP e ∷ tid @ E {{ Φ }}.
   Proof.
     iIntros "H".
     iApply (wp_strong_mono with "H"); first done.
     iSteps.
   Qed.
 
-  Lemma wp_atomic e `{!Atomic e} E1 E2 Φ :
-    (|={E1, E2}=> WP e @ E2 {{ v, |={E2, E1}=> Φ v }}) ⊢
-    WP e @ E1 {{ Φ }}.
-  Proof.
-    iIntros "H".
-    rewrite !wp_unfold /wp_pre.
-    destruct (to_val e) as [v |] eqn:He; first iSteps.
-    iIntros "%nt %σ1 %κ1 %κs Hσ".
-    iMod "H".
-    iMod ("H" with "Hσ") as "($ & H)".
-    iModIntro. iIntros "%e2 %σ2 %es1 %Hstep1 H£".
-    iMod ("H" with "[//] H£") as "H".
-    do 2 iModIntro.
-    iMod "H" as "(Hσ & H & Hes)".
-    rewrite !wp_unfold /wp_pre.
-    destruct (to_val e2) as [v2 |] eqn:He2.
-    - iDestruct "H" as ">>$".
-      iSteps.
-    - iMod ("H" $! _ _ [] with "Hσ") as "(%Hreducible2 & _)".
-      destruct Hreducible2 as (κ2 & e3 & σ3 & es2 & Hstep2).
-      edestruct atomic; [done | congruence].
-  Qed.
-
-  Lemma wp_step_fupd e E1 E2 P Φ :
-    TCEq (to_val e) None →
-    E2 ⊆ E1 →
-    (|={E1}[E2]▷=> P) -∗
-    WP e @ E2 {{ v, P ={E1}=∗ Φ v }} -∗
-    WP e @ E1 {{ Φ }}.
-  Proof.
-    rewrite !wp_unfold /wp_pre /=.
-    iIntros (-> HE) "HP H %nt %σ1 %κ1 %κs Hσ".
-    iMod "HP".
-    iMod ("H" with "Hσ") as "($ & H)".
-    iIntros "!> %e2 %σ2 %es1 %Hstep H£".
-    iMod ("H" with "[//] H£") as "H".
-    do 2 iModIntro.
-    iMod "H" as "($ & H & $)".
-    iMod "HP".
-    iApply (wp_strong_mono with "H"); first done.
-    iSteps.
-  Qed.
-
-  Lemma wp_bind K `{!LanguageCtx K} e E Φ :
-    WP e @ E {{ v, WP K (of_val v) @ E {{ Φ }} }} ⊢
-    WP K e @ E {{ Φ }}.
-  Proof.
-    iIntros "H".
-    iLöb as "IH" forall (e).
-    rewrite wp_unfold /wp_pre.
-    destruct (to_val e) as [v |] eqn:He.
-    - apply of_to_val in He as <-.
-      iApply (fupd_wp with "H").
-    - rewrite wp_unfold /wp_pre fill_not_val //.
-      iIntros "%nt %σ1 %κ1 %κs Hσ".
-      iMod ("H" with "Hσ") as "(%Hreducible1 & H)".
-      iModIntro; iSplit; first eauto using reducible_fill.
-      iIntros "%e2 %σ2 %es1 %Hstep1 H£".
-      destruct (fill_step_inv e σ1 κ1 e2 σ2 es1) as (e2' & -> & Hstep1'); [done.. |].
-      iMod ("H" with "[//] H£") as "H".
-      iModIntro. iSteps.
-  Qed.
-
-  Lemma wp_bind_inv K `{!LanguageCtx K} e E Φ :
-    WP K e @ E {{ Φ }} ⊢
-    WP e @ E {{ v, WP K (of_val v) @ E {{ Φ }} }}.
-  Proof.
-    iIntros "H".
-    iLöb as "IH" forall (e).
-    rewrite !wp_unfold /wp_pre /=.
-    destruct (to_val e) as [v |] eqn:He.
-    - apply of_to_val in He as <-.
-      rewrite !wp_unfold /wp_pre //.
-    - rewrite fill_not_val //.
-      iIntros "%nt %σ1 %κ1 %κs Hσ".
-      iMod ("H" with "Hσ") as "(%Hreducible & H)".
-      iModIntro; iSplit; first eauto using reducible_fill_inv.
-      iIntros "%e2 %σ2 %es1 %Hstep1 H£".
-      iMod ("H" with "[] H£") as "H"; first eauto using fill_step.
-      iModIntro. iSteps.
-  Qed.
-
-  Lemma wp_frame_l e E Φ R :
-    R ∗ WP e @ E {{ Φ }} ⊢
-    WP e @ E {{ v, R ∗ Φ v }}.
+  Lemma wp_frame_l e tid E Φ R :
+    R ∗ WP e ∷ tid @ E {{ Φ }} ⊢
+    WP e ∷ tid @ E {{ v, R ∗ Φ v }}.
   Proof.
     iIntros "(HR & H)".
     iApply (wp_strong_mono with "H"); first done.
     iSteps.
   Qed.
-  Lemma wp_frame_r e E Φ R :
-    WP e @ E {{ Φ }} ∗ R ⊢
-    WP e @ E {{ v, Φ v ∗ R }}.
+  Lemma wp_frame_r e tid E Φ R :
+    WP e ∷ tid @ E {{ Φ }} ∗ R ⊢
+    WP e ∷ tid @ E {{ v, Φ v ∗ R }}.
   Proof.
     iIntros "(H & HR)".
     iApply (wp_strong_mono with "H"); first done.
     iSteps.
   Qed.
 
-  Lemma wp_wand e E Φ1 Φ2 :
-    WP e @ E {{ Φ1 }} -∗
+  Lemma wp_wand {e tid E} Φ1 Φ2 :
+    WP e ∷ tid @ E {{ Φ1 }} -∗
     (∀ v, Φ1 v -∗ Φ2 v) -∗
-    WP e @ E {{ Φ2 }}.
+    WP e ∷ tid @ E {{ Φ2 }}.
   Proof.
     iIntros "H HΦ".
     iApply (wp_strong_mono with "H"); first done.
     iSteps.
   Qed.
-  Lemma wp_wand_l e E Φ1 Φ2 :
-    (∀ v, Φ1 v -∗ Φ2 v) ∗ WP e @ E {{ Φ1 }} ⊢
-    WP e @ E {{ Φ2 }}.
-  Proof.
-    iIntros "(HΦ & H)".
-    iApply (wp_wand with "H HΦ").
-  Qed.
-  Lemma wp_wand_r e E Φ1 Φ2 :
-    WP e @ E {{ Φ1 }} ∗ (∀ v, Φ1 v -∗ Φ2 v) ⊢
-    WP e @ E {{ Φ2 }}.
-  Proof.
-    iIntros "(H & HΦ)".
-    iApply (wp_wand with "H HΦ").
-  Qed.
-  Lemma wp_frame_wand e E Φ R :
+  Lemma wp_frame_wand e tid E Φ R :
     R -∗
-    WP e @ E {{ v, R -∗ Φ v }} -∗
-    WP e @ E {{ Φ }}.
+    WP e ∷ tid @ E {{ v, R -∗ Φ v }} -∗
+    WP e ∷ tid @ E {{ Φ }}.
   Proof.
     iIntros "HR H".
     iApply (wp_wand with "H").
     iSteps.
   Qed.
 
-  #[global] Instance frame_wp p e E R Φ1 Φ2 :
+  Lemma wp_atomic e `{!Atomic e} tid E1 E2 Φ :
+    (|={E1,E2}=> WP e ∷ tid @ E2 {{ v, |={E2,E1}=> Φ v }}) ⊢
+    WP e ∷ tid @ E1 {{ Φ }}.
+  Proof.
+    wp_unseal.
+    - apply bwp_atomic; first done.
+    - iIntros "H %tid".
+      iSpecialize ("H" $! tid).
+      iApply (bwp_atomic with "H").
+  Qed.
+
+  Lemma wp_step_fupd e tid E1 E2 P Φ :
+    TCEq (to_val e) None →
+    E2 ⊆ E1 →
+    (|={E1}[E2]▷=> P) -∗
+    WP e ∷ tid @ E2 {{ v, P ={E1}=∗ Φ v }} -∗
+    WP e ∷ tid @ E1 {{ Φ }}.
+  Proof.
+    wp_unseal.
+    - apply bwp_step_fupd.
+    - iIntros "%He %HE HP H %tid".
+      iApply (bwp_step_fupd with "HP H"); first done.
+  Qed.
+
+  Lemma wp_bind K `{!LanguageCtx K} e tid1 tid2 E Φ :
+    ( if tid2 is Some tid2 then
+        if tid1 is Some tid1 then
+          tid1 = tid2
+        else
+          False
+      else
+        True
+    ) →
+    WP e ∷ tid2 @ E {{ v, WP K (of_val v) ∷ tid1 @ E {{ Φ }} }} ⊢
+    WP K e ∷ tid1 @ E {{ Φ }}.
+  Proof.
+    wp_unseal; destruct tid1 as [tid1 |].
+    - intros ->.
+      apply bwp_bind; first done.
+    - done.
+    - iIntros "_ H".
+      iApply (bwp_bind with "H").
+    - iIntros "_ H %tid".
+      iApply bwp_bind.
+      iApply (bwp_wand with "H").
+      iSteps.
+  Qed.
+  Lemma wp_bind' K `{!LanguageCtx K} e tid E Φ :
+    WP e ∷ tid @ E {{ v, WP K (of_val v) ∷ tid @ E {{ Φ }} }} ⊢
+    WP K e ∷ tid @ E {{ Φ }}.
+  Proof.
+    apply: wp_bind.
+    destruct tid; done.
+  Qed.
+
+  #[global] Instance frame_wp p e tid E R Φ1 Φ2 :
     (∀ v, Frame p R (Φ1 v) (Φ2 v)) →
     Frame
       p
       R
-      (WP e @ E {{ Φ1 }})
-      (WP e @ E {{ Φ2 }})
+      (WP e ∷ tid @ E {{ Φ1 }})
+      (WP e ∷ tid @ E {{ Φ2 }})
   | 2.
   Proof.
     rewrite /Frame wp_frame_l => HR.
     apply wp_mono, HR.
   Qed.
 
-  #[global] Instance is_except_0_wp e E Φ :
-    IsExcept0 (WP e @ E {{ Φ }}).
+  #[global] Instance is_except_0_wp e tid E Φ :
+    IsExcept0 (WP e ∷ tid @ E {{ Φ }}).
   Proof.
     rewrite /IsExcept0 -{2}fupd_wp -except_0_fupd -fupd_intro //.
   Qed.
 
-  #[global] Instance elim_modal_bupd_wp p e E P Φ :
+  #[global] Instance elim_modal_bupd_wp p e tid E P Φ :
     ElimModal
       True
       p
       false
       (|==> P)
       P
-      (WP e @ E {{ Φ }})
-      (WP e @ E {{ Φ }}).
+      (WP e ∷ tid @ E {{ Φ }})
+      (WP e ∷ tid @ E {{ Φ }}).
   Proof.
     rewrite /ElimModal bi.intuitionistically_if_elim (bupd_fupd E) fupd_frame_r bi.wand_elim_r fupd_wp //.
   Qed.
 
-  #[global] Instance elim_modal_fupd_wp p e E P Φ :
+  #[global] Instance elim_modal_fupd_wp p e tid E P Φ :
     ElimModal
       True
       p
       false
       (|={E}=> P)
       P
-      (WP e @ E {{ Φ }})
-      (WP e @ E {{ Φ }}).
+      (WP e ∷ tid @ E {{ Φ }})
+      (WP e ∷ tid @ E {{ Φ }}).
   Proof.
     rewrite /ElimModal bi.intuitionistically_if_elim fupd_frame_r bi.wand_elim_r fupd_wp //.
   Qed.
-  #[global] Instance elim_modal_fupd_wp_wrong_mask p e E1 E2 P Φ :
+  #[global] Instance elim_modal_fupd_wp_wrong_mask p e tid E1 E2 P Φ :
     ElimModal
       (pm_error "Goal and eliminated modality must have the same mask.
 Use [iApply fupd_wp; iMod (fupd_mask_subseteq E2)] to adjust the mask of your goal to [E2]")
@@ -485,28 +393,28 @@ Use [iApply fupd_wp; iMod (fupd_mask_subseteq E2)] to adjust the mask of your go
       false
       (|={E2}=> P)
       False
-      (WP e @ E1 {{ Φ }})
+      (WP e ∷ tid @ E1 {{ Φ }})
       False
   | 100.
   Proof.
     intros [].
   Qed.
 
-  #[global] Instance elim_modal_fupd_wp_atomic p e E1 E2 P Φ :
+  #[global] Instance elim_modal_fupd_wp_atomic p e tid E1 E2 P Φ :
     ElimModal
       (Atomic e)
       p
       false
       (|={E1,E2}=> P)
       P
-      (WP e @ E1 {{ Φ }})
-      (WP e @ E2 {{ v, |={E2,E1}=> Φ v }})%I
+      (WP e ∷ tid @ E1 {{ Φ }})
+      (WP e ∷ tid @ E2 {{ v, |={E2,E1}=> Φ v }})%I
   | 100.
   Proof.
     intros He.
     rewrite bi.intuitionistically_if_elim fupd_frame_r bi.wand_elim_r wp_atomic //.
   Qed.
-  #[global] Instance elim_modal_fupd_wp_atomic_wrong_mask p e E1 E2 E2' P Φ :
+  #[global] Instance elim_modal_fupd_wp_atomic_wrong_mask p e tid E1 E2 E2' P Φ :
     ElimModal
       (pm_error "Goal and eliminated modality must have the same mask.
 Use [iMod (fupd_mask_subseteq E2)] to adjust the mask of your goal to [E2]")
@@ -514,23 +422,23 @@ Use [iMod (fupd_mask_subseteq E2)] to adjust the mask of your goal to [E2]")
       false
       (|={E2,E2'}=> P)
       False
-      (WP e @ E1 {{ Φ }})
+      (WP e ∷ tid @ E1 {{ Φ }})
       False
   | 200.
   Proof.
     intros [].
   Qed.
 
-  #[global] Instance add_modal_fupd_wp e E P Φ :
+  #[global] Instance add_modal_fupd_wp e tid E P Φ :
     AddModal
       (|={E}=> P)
       P
-      (WP e @ E {{ Φ }}).
+      (WP e ∷ tid @ E {{ Φ }}).
   Proof.
     rewrite /AddModal fupd_frame_r bi.wand_elim_r fupd_wp //.
   Qed.
 
-  #[global] Instance elim_acc_wp_atomic {X} e E1 E2 α β γ Φ :
+  #[global] Instance elim_acc_wp_atomic {X} e tid E1 E2 α β γ Φ :
     ElimAcc (X := X)
       (Atomic e)
       (fupd E1 E2)
@@ -538,8 +446,8 @@ Use [iMod (fupd_mask_subseteq E2)] to adjust the mask of your goal to [E2]")
       α
       β
       γ
-      (WP e @ E1 {{ Φ }})
-      (λ x, WP e @ E2 {{ v, |={E2}=> β x ∗ (γ x -∗? Φ v) }})%I
+      (WP e ∷ tid @ E1 {{ Φ }})
+      (λ x, WP e ∷ tid @ E2 {{ v, |={E2}=> β x ∗ (γ x -∗? Φ v) }})%I
   | 100.
   Proof.
     iIntros "%He Hinner >Hacc".
@@ -548,7 +456,7 @@ Use [iMod (fupd_mask_subseteq E2)] to adjust the mask of your goal to [E2]")
     iApply ("HΦ" with "(Hclose Hβ)").
   Qed.
 
-  #[global] Instance elim_acc_wp_nonatomic {X} e E α β γ Φ :
+  #[global] Instance elim_acc_wp_nonatomic {X} e tid E α β γ Φ :
     ElimAcc (X := X)
       True
       (fupd E E)
@@ -556,13 +464,36 @@ Use [iMod (fupd_mask_subseteq E2)] to adjust the mask of your goal to [E2]")
       α
       β
       γ
-      (WP e @ E {{ Φ }})
-      (λ x, WP e @ E {{ v, |={E}=> β x ∗ (γ x -∗? Φ v) }})%I.
+      (WP e ∷ tid @ E {{ Φ }})
+      (λ x, WP e ∷ tid @ E {{ v, |={E}=> β x ∗ (γ x -∗? Φ v) }})%I.
   Proof.
     iIntros (_) "Hinner >Hacc".
     iDestruct "Hacc" as "(%x & Hα & Hclose)".
     iApply wp_fupd.
     iApply (wp_wand with "(Hinner Hα)"). iIntros "%v >(Hβ & HΦ)".
     iApply ("HΦ" with "(Hclose Hβ)").
+  Qed.
+End iris_G.
+
+Section iris_G.
+  Context `{iris_G : !IrisG Λ Σ}.
+
+  Implicit Types e : expr Λ.
+  Implicit Types Φ : val Λ → iProp Σ.
+
+  Lemma wp_pure_step_later `{!Inhabited (state Λ)} ϕ n e1 e2 tid E Φ :
+    PureExec ϕ n e1 e2 →
+    ϕ →
+    ▷^n (
+      £ n -∗
+      WP e2 ∷ tid @ E {{ Φ }}
+    ) ⊢
+    WP e1 ∷ tid @ E {{ Φ }}.
+  Proof.
+    wp_unseal.
+    - apply bwp_pure_step_later.
+    - iIntros "%Hexec %Hϕ H %tid".
+      iApply bwp_pure_step_later; first done.
+      iSteps.
   Qed.
 End iris_G.
