theories/zoo/iris/program_logic/bwp.v
@@ -1,0 +1,844 @@
+From iris.base_logic Require Export
+  lib.fancy_updates.
+
+From zoo Require Import
+  prelude.
+From zoo.iris Require Import
+  diaframe.
+From zoo.iris.program_logic Require Export
+  language.
+From zoo Require Import
+  options.
+
+Class IrisG Λ Σ := {
+  #[global] iris_G_inv_G :: invGS Σ ;
+  state_interp : nat → state Λ → list (observation Λ) → iProp Σ ;
+  fork_post : val Λ → iProp Σ ;
+}.
+#[global] Arguments Build_IrisG {_ _ _} _ _ : assert.
+#[global] Opaque iris_G_inv_G.
+
+Section iris_G.
+  Context `{iris_G : !IrisG Λ Σ}.
+
+  Definition bwp_pre (bwp : expr Λ -d> thread_id -d> coPset -d> (val Λ -d> iPropO Σ) -d> iPropO Σ)
+  : expr Λ -d> thread_id -d> coPset -d> (val Λ -d> iPropO Σ) -d> iPropO Σ
+  :=
+    λ e tid E Φ,
+      match to_val e with
+      | Some v =>
+          |={E}=> Φ v
+      | None =>
+          ∀ nt σ κ κs,
+          state_interp nt σ (κ ++ κs) -∗
+            |={E,∅}=>
+            ⌜reducible tid e σ⌝ ∗
+              ∀ e' σ' es,
+              ⌜prim_step tid e σ κ e' σ' es⌝ -∗
+              £ 1 -∗
+                |={∅}=> ▷ |={∅,E}=>
+                state_interp (nt + length es) σ' κs ∗
+                bwp e' tid E Φ ∗
+                [∗ list] i ↦ e ∈ es,
+                  bwp e (nt + i) ⊤ fork_post
+      end%I.
+  #[global] Arguments bwp_pre bwp e%_E tid E Φ%_I : rename.
+
+  #[local] Instance bwp_pre_contractive :
+    Contractive bwp_pre.
+  Proof.
+    rewrite /bwp_pre /= => n bwp1 bwp2 Hbwp e tid E Φ.
+    repeat (apply Hbwp || f_contractive || f_equiv).
+  Qed.
+
+  #[local] Definition bwp_def :=
+    fixpoint bwp_pre.
+  #[global] Arguments bwp_def e%_E tid E Φ%_I : rename.
+End iris_G.
+
+#[local] Definition bwp_aux : seal (@bwp_def).
+  Proof. by eexists. Qed.
+Definition bwp :=
+  bwp_aux.(unseal).
+#[global] Arguments bwp {_ _ _} e%_E tid E Φ%_I : rename.
+#[local] Lemma bwp_unseal `{iris_G : !IrisG Λ Σ} :
+  bwp = @bwp_def Λ Σ _.
+Proof.
+  rewrite -bwp_aux.(seal_eq) //.
+Qed.
+
+Declare Custom Entry wp_mask.
+Notation "" := (
+  @top coPset _
+)(in custom wp_mask
+).
+Notation "@ E" :=
+  E
+( in custom wp_mask at level 200,
+  E constr,
+  format "'/  ' @  E "
+).
+
+Notation "'BWP' e ∶ tid E {{ Φ } }" := (
+  bwp e%E tid E Φ%I
+)(at level 20,
+  e at level 200,
+  tid at level 200,
+  E custom wp_mask at level 200,
+  Φ at level 200,
+  format "'[hv' BWP  '/  ' '[' e ']'  '/  ' ∶  tid  E '/' {{  '[' Φ ']'  '/' } } ']'"
+) : bi_scope.
+Notation "'BWP' e ∶ tid E {{ v , Q } }" := (
+  bwp e%E tid E (λ v, Q%I)
+)(at level 20,
+  e at level 200,
+  tid at level 200,
+  E custom wp_mask at level 200,
+  Q at level 200,
+  v at level 200 as pattern,
+  format "'[hv' BWP  '/  ' '[' e ']'  '/  ' ∶  tid  E '/' {{  '[' v ,  '/' Q ']'  '/' } } ']'"
+) : bi_scope.
+
+Section iris_G.
+  Context `{iris_G : !IrisG Λ Σ}.
+
+  Implicit Types e : expr Λ.
+  Implicit Types v : val Λ.
+  Implicit Types P R : iProp Σ.
+  Implicit Types Φ : val Λ → iProp Σ.
+
+  Lemma bwp_unfold e tid E Φ :
+    BWP e ∶ tid @ E {{ Φ }} ⊣⊢
+    bwp_pre bwp e tid E Φ.
+  Proof.
+    rewrite bwp_unseal. apply (fixpoint_unfold bwp_pre).
+  Qed.
+
+  #[global] Instance bwp_ne n e tid E :
+    Proper (pointwise_relation _ (≡{n}≡) ==> (≡{n}≡)) (bwp e tid E).
+  Proof.
+    move: e. induction (lt_wf n) as [n _ IH] => e Φ1 Φ2 HΦ.
+    rewrite !bwp_unfold /bwp_pre /=.
+    do 25 (f_contractive || f_equiv).
+    apply IH; first done.
+    f_equiv.
+    eapply dist_le; [apply HΦ | lia].
+  Qed.
+  #[global] Instance bwp_proper e tid E :
+    Proper (pointwise_relation _ (≡) ==> (≡)) (bwp e tid E).
+  Proof.
+    intros Φ1 Φ2 HΦ.
+    apply equiv_dist => n. apply bwp_ne => v. apply equiv_dist. done.
+  Qed.
+  #[global] Instance bwp_contractive n e tid E :
+    TCEq (to_val e) None →
+    Proper (pointwise_relation _ (dist_later n) ==> (≡{n}≡)) (bwp e tid E).
+  Proof.
+    intros He Φ1 Φ2 HΦ.
+    rewrite !bwp_unfold /bwp_pre He /=.
+    repeat (f_contractive || f_equiv).
+  Qed.
+
+  Lemma bwp_value_fupd' v tid E Φ :
+    BWP of_val v ∶ tid @ E {{ Φ }} ⊣⊢
+    |={E}=> Φ v.
+  Proof.
+    rewrite bwp_unfold /bwp_pre to_of_val //.
+  Qed.
+  Lemma bwp_value_fupd e v tid E Φ :
+    AsVal e v →
+    BWP e ∶ tid @ E {{ Φ }} ⊣⊢
+    |={E}=> Φ v.
+  Proof.
+    rewrite -bwp_value_fupd' => <- //.
+  Qed.
+  Lemma bwp_value' v tid E Φ :
+    Φ v ⊢
+    BWP of_val v ∶ tid @ E {{ Φ }}.
+  Proof.
+    rewrite bwp_value_fupd'. auto.
+  Qed.
+  Lemma bwp_value e v tid E Φ :
+    AsVal e v →
+    Φ v ⊢
+    BWP e ∶ tid @ E {{ Φ }}.
+  Proof.
+    rewrite bwp_value' => <- //.
+  Qed.
+
+  Lemma bwp_strong_mono e tid E1 Φ1 E2 Φ2 :
+    E1 ⊆ E2 →
+    BWP e ∶ tid @ E1 {{ Φ1 }} -∗
+    (∀ v, Φ1 v ={E2}=∗ Φ2 v) -∗
+    BWP e ∶ tid @ E2 {{ Φ2 }}.
+  Proof.
+    iIntros "%HE H HΦ".
+    iLöb as "HLöb" forall (e).
+    rewrite !bwp_unfold /bwp_pre /=.
+    destruct (to_val e) as [v |] eqn:He.
+    - iApply ("HΦ" with "[> H]").
+      iSteps.
+    - iIntros "%nt %σ1 %κ %κs Hσ".
+      iMod (fupd_mask_subseteq E1) as "Hclose"; first done.
+      iMod ("H" with "Hσ") as "(%Hreducible & H)".
+      iModIntro. iStep. iIntros "%e2 %σ2 %es %Hstep H£".
+      iMod ("H" with "[//] H£") as "H".
+      do 2 iModIntro.
+      iMod "H" as "($ & H & Hes)".
+      iMod "Hclose" as "_".
+      iSplitR "Hes"; iSteps.
+  Qed.
+  Lemma bwp_mono e tid E Φ1 Φ2 :
+    (∀ v, Φ1 v ⊢ Φ2 v) →
+    BWP e ∶ tid @ E {{ Φ1 }} ⊢
+    BWP e ∶ tid @ E {{ Φ2 }}.
+  Proof.
+    iIntros "%HΦ H".
+    iApply (bwp_strong_mono with "H"); first done. iIntros "%v HΦ".
+    iApply (HΦ with "HΦ").
+  Qed.
+  #[global] Instance bwp_mono' e tid E :
+    Proper (pointwise_relation _ (⊢) ==> (⊢)) (bwp e tid E).
+  Proof.
+    intros Φ1 Φ2 HΦ.
+    apply bwp_mono. done.
+  Qed.
+  #[global] Instance bwp_flip_mono' e tid E :
+    Proper (pointwise_relation _ (flip (⊢)) ==> (flip (⊢))) (bwp e tid E).
+  Proof.
+    solve_proper.
+  Qed.
+
+  Lemma fupd_bwp e tid E Φ :
+    (|={E}=> BWP e ∶ tid @ E {{ Φ }}) ⊢
+    BWP e ∶ tid @ E {{ Φ }}.
+  Proof.
+    iIntros "H".
+    rewrite bwp_unfold /bwp_pre.
+    destruct (to_val e) as [v |] eqn:He; first iSteps.
+    iIntros "%nt %σ1 %κ %κs Hσ".
+    iMod "H".
+    iApply ("H" with "Hσ").
+  Qed.
+  Lemma bwp_fupd e tid E Φ :
+    BWP e ∶ tid @ E {{ v, |={E}=> Φ v }} ⊢
+    BWP e ∶ tid @ E {{ Φ }}.
+  Proof.
+    iIntros "H".
+    iApply (bwp_strong_mono with "H"); first done.
+    iSteps.
+  Qed.
+
+  Lemma bwp_frame_l e tid E Φ R :
+    R ∗ BWP e ∶ tid @ E {{ Φ }} ⊢
+    BWP e ∶ tid @ E {{ v, R ∗ Φ v }}.
+  Proof.
+    iIntros "(HR & H)".
+    iApply (bwp_strong_mono with "H"); first done.
+    iSteps.
+  Qed.
+  Lemma bwp_frame_r e tid E Φ R :
+    BWP e ∶ tid @ E {{ Φ }} ∗ R ⊢
+    BWP e ∶ tid @ E {{ v, Φ v ∗ R }}.
+  Proof.
+    iIntros "(H & HR)".
+    iApply (bwp_strong_mono with "H"); first done.
+    iSteps.
+  Qed.
+
+  Lemma bwp_wand {e tid E} Φ1 Φ2 :
+    BWP e ∶ tid @ E {{ Φ1 }} -∗
+    (∀ v, Φ1 v -∗ Φ2 v) -∗
+    BWP e ∶ tid @ E {{ Φ2 }}.
+  Proof.
+    iIntros "H HΦ".
+    iApply (bwp_strong_mono with "H"); first done.
+    iSteps.
+  Qed.
+  Lemma bwp_frame_wand e tid E Φ R :
+    R -∗
+    BWP e ∶ tid @ E {{ v, R -∗ Φ v }} -∗
+    BWP e ∶ tid @ E {{ Φ }}.
+  Proof.
+    iIntros "HR H".
+    iApply (bwp_wand with "H").
+    iSteps.
+  Qed.
+
+  Lemma bwp_atomic e `{!Atomic e} tid E1 E2 Φ :
+    (|={E1,E2}=> BWP e ∶ tid @ E2 {{ v, |={E2,E1}=> Φ v }}) ⊢
+    BWP e ∶ tid @ E1 {{ Φ }}.
+  Proof.
+    iIntros "H".
+    rewrite !bwp_unfold /bwp_pre.
+    destruct (to_val e) as [v |] eqn:He; first iSteps.
+    iIntros "%nt %σ1 %κ1 %κs Hσ".
+    iMod "H".
+    iMod ("H" with "Hσ") as "($ & H)".
+    iModIntro. iIntros "%e2 %σ2 %es1 %Hstep1 H£".
+    iMod ("H" with "[//] H£") as "H".
+    do 2 iModIntro.
+    iMod "H" as "(Hσ & H & Hes)".
+    rewrite !bwp_unfold /bwp_pre.
+    destruct (to_val e2) as [v2 |] eqn:He2.
+    - iDestruct "H" as ">>$".
+      iSteps.
+    - iMod ("H" $! _ _ [] with "Hσ") as "(%Hreducible2 & _)".
+      destruct Hreducible2 as (κ2 & e3 & σ3 & es2 & Hstep2).
+      edestruct atomic; [done | congruence].
+  Qed.
+
+  Lemma bwp_step_fupd e tid E1 E2 P Φ :
+    TCEq (to_val e) None →
+    E2 ⊆ E1 →
+    (|={E1}[E2]▷=> P) -∗
+    BWP e ∶ tid @ E2 {{ v, P ={E1}=∗ Φ v }} -∗
+    BWP e ∶ tid @ E1 {{ Φ }}.
+  Proof.
+    rewrite !bwp_unfold /bwp_pre /=.
+    iIntros (-> HE) "HP H %nt %σ1 %κ1 %κs Hσ".
+    iMod "HP".
+    iMod ("H" with "Hσ") as "($ & H)".
+    iIntros "!> %e2 %σ2 %es1 %Hstep H£".
+    iMod ("H" with "[//] H£") as "H".
+    do 2 iModIntro.
+    iMod "H" as "($ & H & $)".
+    iMod "HP".
+    iApply (bwp_strong_mono with "H"); first done.
+    iSteps.
+  Qed.
+
+  Lemma bwp_bind K `{!LanguageCtx K} e tid E Φ :
+    BWP e ∶ tid @ E {{ v, BWP K (of_val v) ∶ tid @ E {{ Φ }} }} ⊢
+    BWP K e ∶ tid @ E {{ Φ }}.
+  Proof.
+    iIntros "H".
+    iLöb as "IH" forall (e).
+    rewrite bwp_unfold /bwp_pre.
+    destruct (to_val e) as [v |] eqn:He.
+    - apply of_to_val in He as <-.
+      iApply (fupd_bwp with "H").
+    - rewrite bwp_unfold /bwp_pre fill_not_val //.
+      iIntros "%nt %σ1 %κ1 %κs Hσ".
+      iMod ("H" with "Hσ") as "(%Hreducible1 & H)".
+      iModIntro; iSplit; first eauto using reducible_fill.
+      iIntros "%e2 %σ2 %es1 %Hstep1 H£".
+      destruct (fill_step_inv tid e σ1 κ1 e2 σ2 es1) as (e2' & -> & Hstep1'); [done.. |].
+      iMod ("H" with "[//] H£") as "H".
+      iModIntro. iSteps.
+  Qed.
+
+  Lemma bwp_bind_inv K `{!LanguageCtx K} e tid E Φ :
+    BWP K e ∶ tid @ E {{ Φ }} ⊢
+    BWP e ∶ tid @ E {{ v, BWP K (of_val v) ∶ tid @ E {{ Φ }} }}.
+  Proof.
+    iIntros "H".
+    iLöb as "IH" forall (e).
+    rewrite !bwp_unfold /bwp_pre /=.
+    destruct (to_val e) as [v |] eqn:He.
+    - apply of_to_val in He as <-.
+      rewrite !bwp_unfold /bwp_pre //.
+    - rewrite fill_not_val //.
+      iIntros "%nt %σ1 %κ1 %κs Hσ".
+      iMod ("H" with "Hσ") as "(%Hreducible & H)".
+      iModIntro; iSplit; first eauto using reducible_fill_inv.
+      iIntros "%e2 %σ2 %es1 %Hstep1 H£".
+      iMod ("H" with "[] H£") as "H"; first eauto using fill_step.
+      iModIntro. iSteps.
+  Qed.
+
+  #[global] Instance frame_bwp p e tid E R Φ1 Φ2 :
+    (∀ v, Frame p R (Φ1 v) (Φ2 v)) →
+    Frame
+      p
+      R
+      (BWP e ∶ tid @ E {{ Φ1 }})
+      (BWP e ∶ tid @ E {{ Φ2 }})
+  | 2.
+  Proof.
+    rewrite /Frame bwp_frame_l => HR.
+    apply bwp_mono, HR.
+  Qed.
+
+  #[global] Instance is_except_0_bwp e tid E Φ :
+    IsExcept0 (BWP e ∶ tid @ E {{ Φ }}).
+  Proof.
+    rewrite /IsExcept0 -{2}fupd_bwp -except_0_fupd -fupd_intro //.
+  Qed.
+
+  #[global] Instance elim_modal_bupd_bwp p e tid E P Φ :
+    ElimModal
+      True
+      p
+      false
+      (|==> P)
+      P
+      (BWP e ∶ tid @ E {{ Φ }})
+      (BWP e ∶ tid @ E {{ Φ }}).
+  Proof.
+    rewrite /ElimModal bi.intuitionistically_if_elim (bupd_fupd E) fupd_frame_r bi.wand_elim_r fupd_bwp //.
+  Qed.
+
+  #[global] Instance elim_modal_fupd_bwp p e tid E P Φ :
+    ElimModal
+      True
+      p
+      false
+      (|={E}=> P)
+      P
+      (BWP e ∶ tid @ E {{ Φ }})
+      (BWP e ∶ tid @ E {{ Φ }}).
+  Proof.
+    rewrite /ElimModal bi.intuitionistically_if_elim fupd_frame_r bi.wand_elim_r fupd_bwp //.
+  Qed.
+  #[global] Instance elim_modal_fupd_bwp_wrong_mask p e tid E1 E2 P Φ :
+    ElimModal
+      (pm_error "Goal and eliminated modality must have the same mask.
+Use [iApply fupd_bwp; iMod (fupd_mask_subseteq E2)] to adjust the mask of your goal to [E2]")
+      p
+      false
+      (|={E2}=> P)
+      False
+      (BWP e ∶ tid @ E1 {{ Φ }})
+      False
+  | 100.
+  Proof.
+    intros [].
+  Qed.
+
+  #[global] Instance elim_modal_fupd_bwp_atomic p e tid E1 E2 P Φ :
+    ElimModal
+      (Atomic e)
+      p
+      false
+      (|={E1,E2}=> P)
+      P
+      (BWP e ∶ tid @ E1 {{ Φ }})
+      (BWP e ∶ tid @ E2 {{ v, |={E2,E1}=> Φ v }})%I
+  | 100.
+  Proof.
+    intros He.
+    rewrite bi.intuitionistically_if_elim fupd_frame_r bi.wand_elim_r bwp_atomic //.
+  Qed.
+  #[global] Instance elim_modal_fupd_bwp_atomic_wrong_mask p e tid E1 E2 E2' P Φ :
+    ElimModal
+      (pm_error "Goal and eliminated modality must have the same mask.
+Use [iMod (fupd_mask_subseteq E2)] to adjust the mask of your goal to [E2]")
+      p
+      false
+      (|={E2,E2'}=> P)
+      False
+      (BWP e ∶ tid @ E1 {{ Φ }})
+      False
+  | 200.
+  Proof.
+    intros [].
+  Qed.
+
+  #[global] Instance add_modal_fupd_bwp e tid E P Φ :
+    AddModal
+      (|={E}=> P)
+      P
+      (BWP e ∶ tid @ E {{ Φ }}).
+  Proof.
+    rewrite /AddModal fupd_frame_r bi.wand_elim_r fupd_bwp //.
+  Qed.
+
+  #[global] Instance elim_acc_bwp_atomic {X} e tid E1 E2 α β γ Φ :
+    ElimAcc (X := X)
+      (Atomic e)
+      (fupd E1 E2)
+      (fupd E2 E1)
+      α
+      β
+      γ
+      (BWP e ∶ tid @ E1 {{ Φ }})
+      (λ x, BWP e ∶ tid @ E2 {{ v, |={E2}=> β x ∗ (γ x -∗? Φ v) }})%I
+  | 100.
+  Proof.
+    iIntros "%He Hinner >Hacc".
+    iDestruct "Hacc" as "(%x & Hα & Hclose)".
+    iApply (bwp_wand with "(Hinner Hα)"). iIntros "%v >(Hβ & HΦ)".
+    iApply ("HΦ" with "(Hclose Hβ)").
+  Qed.
+
+  #[global] Instance elim_acc_bwp_nonatomic {X} e tid E α β γ Φ :
+    ElimAcc (X := X)
+      True
+      (fupd E E)
+      (fupd E E)
+      α
+      β
+      γ
+      (BWP e ∶ tid @ E {{ Φ }})
+      (λ x, BWP e ∶ tid @ E {{ v, |={E}=> β x ∗ (γ x -∗? Φ v) }})%I.
+  Proof.
+    iIntros (_) "Hinner >Hacc".
+    iDestruct "Hacc" as "(%x & Hα & Hclose)".
+    iApply bwp_fupd.
+    iApply (bwp_wand with "(Hinner Hα)"). iIntros "%v >(Hβ & HΦ)".
+    iApply ("HΦ" with "(Hclose Hβ)").
+  Qed.
+End iris_G.
+
+Section iris_G.
+  Context `{iris_G : !IrisG Λ Σ}.
+
+  Implicit Types e : expr Λ.
+  Implicit Types Φ : val Λ → iProp Σ.
+
+  Lemma bwp_lift_step e tid E Φ :
+    to_val e = None →
+    ( ∀ nt σ κ κs,
+      state_interp nt σ (κ ++ κs) -∗
+        |={E, ∅}=>
+        ⌜reducible tid e σ⌝ ∗
+          ∀ e' σ' es,
+          ⌜prim_step tid e σ κ e' σ' es⌝ -∗
+          £ 1 -∗
+            |={∅}=> ▷ |={∅, E}=>
+            state_interp (nt + length es) σ' κs ∗
+            BWP e' ∶ tid @ E {{ Φ }} ∗
+            [∗ list] i ↦ e ∈ es,
+              BWP e ∶ nt + i {{ fork_post }}
+    ) ⊢
+    BWP e ∶ tid @ E {{ Φ }}.
+  Proof.
+    rewrite bwp_unfold /bwp_pre => -> //.
+  Qed.
+  Lemma bwp_lift_step_nofork e tid E Φ :
+    to_val e = None →
+    ( ∀ nt σ κ κs,
+      state_interp nt σ (κ ++ κs) -∗
+        |={E, ∅}=>
+        ⌜reducible tid e σ⌝ ∗
+          ∀ e' σ' es,
+          ⌜prim_step tid e σ κ e' σ' es⌝ -∗
+          £ 1 -∗
+            |={∅}=> ▷ |={∅, E}=>
+            ⌜es = []⌝ ∗
+            state_interp nt σ' κs ∗
+            BWP e' ∶ tid @ E {{ Φ }}
+    ) ⊢
+    BWP e ∶ tid @ E {{ Φ }}.
+  Proof.
+    iIntros "%He H".
+    iApply bwp_lift_step; first done. iIntros "%nt %σ %κ %κs Hσ".
+    iMod ("H" with "Hσ") as "($ & H)".
+    iIntros "!> %e' %σ' %es %Hstep H£".
+    iMod ("H" with "[//] H£") as "H".
+    do 2 iModIntro.
+    iMod "H" as "(-> & Hσ & H)".
+    rewrite Nat.add_0_r. iSteps.
+  Qed.
+
+  Lemma bwp_lift_atomic_step e tid E1 E2 Φ :
+    to_val e = None →
+    ( ∀ nt σ κ κs,
+      state_interp nt σ (κ ++ κs) -∗
+        |={E1}=>
+        ⌜reducible tid e σ⌝ ∗
+          ∀ e' σ' es,
+          ⌜prim_step tid e σ κ e' σ' es⌝ -∗
+          £ 1 -∗
+            |={E1}[E2]▷=>
+            state_interp (nt + length es) σ' κs ∗
+            from_option Φ False (to_val e') ∗
+            [∗ list] i ↦ e ∈ es,
+              BWP e ∶ nt + i {{ fork_post }}
+    ) ⊢
+    BWP e ∶ tid @ E1 {{ Φ }}.
+  Proof.
+    iIntros "%He H".
+    iApply bwp_lift_step; first done. iIntros "%nt %σ %κ %κs Hσ".
+    iMod ("H" with "Hσ") as "($ & H)".
+    iApply fupd_mask_intro; first set_solver. iIntros "Hclose %e' %σ' %es %Hstep H£".
+    iMod "Hclose" as "_".
+    iMod ("H" with "[//] H£") as "H".
+    iApply fupd_mask_intro; first set_solver. iIntros "Hclose !>".
+    iMod "Hclose" as "_".
+    iMod "H" as "($ & HΦ & $)".
+    destruct (to_val e') eqn:He'; last by iExFalso.
+    iApply (bwp_value with "HΦ").
+    apply of_to_val. done.
+  Qed.
+  Lemma bwp_lift_atomic_step_nofork e tid E1 E2 Φ :
+    to_val e = None →
+    ( ∀ nt σ κ κs,
+      state_interp nt σ (κ ++ κs) -∗
+        |={E1}=>
+        ⌜reducible tid e σ⌝ ∗
+          ∀ e' σ' es,
+          ⌜prim_step tid e σ κ e' σ' es⌝ -∗
+          £ 1 -∗
+            |={E1}[E2]▷=>
+            ⌜es = []⌝ ∗
+            state_interp nt σ' κs ∗
+            from_option Φ False (to_val e')
+    ) ⊢
+    BWP e ∶ tid @ E1 {{ Φ }}.
+  Proof.
+    iIntros "%He H".
+    iApply bwp_lift_atomic_step; first done. iIntros "%nt %σ %κ %κs Hσ".
+    iMod ("H" with "Hσ") as "($ & H)".
+    iIntros "!> %e' %σ' %es %Hstep H£".
+    iMod ("H" with "[//] H£") as "H".
+    do 2 iModIntro.
+    iMod "H" as "(-> & Hσ & H)".
+    rewrite Nat.add_0_r. iSteps.
+  Qed.
+
+  Lemma bwp_lift_pure_step_nofork `{!Inhabited (state Λ)} e tid E1 E2 Φ :
+    ( ∀ σ,
+      reducible tid e σ
+    ) →
+    ( ∀ σ κ e' σ' es,
+      prim_step tid e σ κ e' σ' es →
+        κ = [] ∧
+        σ' = σ ∧
+        es = []
+    ) →
+    ( |={E1}[E2]▷=>
+      ∀ σ e' κ es,
+      ⌜prim_step tid e σ κ e' σ es⌝ -∗
+      £ 1 -∗
+      BWP e' ∶ tid @ E1 {{ Φ }}
+    ) ⊢
+    BWP e ∶ tid @ E1 {{ Φ }}.
+  Proof.
+    iIntros "%Hsafe %Hpure H".
+    iApply bwp_lift_step.
+    { specialize (Hsafe inhabitant). eauto using reducible_not_val. }
+    iIntros "%nt %σ %κ %κs Hσ".
+    iMod "H".
+    iApply fupd_mask_intro; first set_solver. iIntros "Hclose".
+    iSplit; first iSteps. iIntros "%e' %σ' %es %Hstep H£ !> !>".
+    edestruct Hpure as (? & ? & ?); first done. subst.
+    rewrite Nat.add_0_r. iSteps.
+  Qed.
+
+  Lemma bwp_lift_pure_det_step_nofork `{!Inhabited (state Λ)} e1 e2 tid E1 E2 Φ :
+    ( ∀ σ1,
+      reducible tid e1 σ1
+    ) →
+    ( ∀ σ1 κ e2' σ2 es,
+      prim_step tid e1 σ1 κ e2' σ2 es →
+        κ = [] ∧
+        σ2 = σ1 ∧
+        e2' = e2 ∧
+        es = []
+    ) →
+    ( |={E1}[E2]▷=>
+      £ 1 -∗
+      BWP e2 ∶ tid @ E1 {{ Φ }}
+    ) ⊢
+    BWP e1 ∶ tid @ E1 {{ Φ }}.
+  Proof.
+    iIntros "%Hsafe %Hpure H".
+    iApply (bwp_lift_pure_step_nofork); [done | naive_solver |].
+    iApply (step_fupd_wand with "H"). iIntros "H %σ1 %e2' %κ %es %Hstep H£".
+    apply Hpure in Hstep as (-> & _ & -> & ->).
+    iSteps.
+  Qed.
+
+  Lemma bwp_pure_step `{!Inhabited (state Λ)} ϕ n e1 e2 tid E1 E2 Φ :
+    PureExec ϕ n e1 e2 →
+    ϕ →
+    ( |={E1}[E2]▷=>^n
+      £ n -∗
+      BWP e2 ∶ tid @ E1 {{ Φ }}
+    ) ⊢
+    BWP e1 ∶ tid @ E1 {{ Φ }}.
+  Proof.
+    iIntros "%Hexec %Hϕ H".
+    specialize (Hexec Hϕ).
+    iInduction Hexec as [e | n e1 e2 e3 (Hsafe & Hpure)] "IH" => /=.
+    - iMod lc_zero as "H£".
+      iSteps.
+    - iApply bwp_lift_pure_det_step_nofork.
+      + eauto using reducible_no_obs_reducible.
+      + naive_solver.
+      + iApply (step_fupd_wand with "H"). iIntros "H H£".
+        iApply "IH".
+        iApply (step_fupdN_wand with "H").
+        rewrite (lc_succ n). iSteps.
+  Qed.
+  Lemma bwp_pure_step_later `{!Inhabited (state Λ)} ϕ n tid e1 e2 E Φ :
+    PureExec ϕ n e1 e2 →
+    ϕ →
+    ▷^n (
+      £ n -∗
+      BWP e2 ∶ tid @ E {{ Φ }}
+    ) ⊢
+    BWP e1 ∶ tid @ E {{ Φ }}.
+  Proof.
+    intros Hexec Hϕ.
+    rewrite -bwp_pure_step // {Hexec}.
+    enough (∀ P, ▷^n P ⊢ |={E}▷=>^n P) as H by apply H.
+    intros P. induction n as [| n IH]; rewrite //= -step_fupd_intro // IH //.
+  Qed.
+End iris_G.
+
+From zoo.iris.program_logic Require Import
+  ectx_language.
+
+Section iris_G.
+  Context {Λ : ectx_language} `{iris_G : !IrisG Λ Σ}.
+
+  Implicit Types e : expr Λ.
+  Implicit Types Φ : val Λ → iProp Σ.
+
+  #[local] Hint Resolve
+    base_reducible_reducible
+    base_reducible_prim_step
+  : core.
+
+  Lemma bwp_lift_base_step e tid E Φ :
+    to_val e = None →
+    ( ∀ nt σ κ κs,
+      state_interp nt σ (κ ++ κs) -∗
+        |={E, ∅}=>
+        ⌜base_reducible tid e σ⌝ ∗
+          ∀ e' σ' es,
+          ⌜base_step tid e σ κ e' σ' es⌝ -∗
+          £ 1 -∗
+            |={∅}=> ▷ |={∅, E}=>
+            state_interp (nt + length es) σ' κs ∗
+            BWP e' ∶ tid @ E {{ Φ }} ∗
+            [∗ list] i ↦ e ∈ es,
+              BWP e ∶ nt + i {{ fork_post }}
+    ) ⊢
+    BWP e ∶ tid @ E {{ Φ }}.
+  Proof.
+    iIntros "%He H".
+    iApply bwp_lift_step; first done. iIntros "%nt %σ %κ %κs Hσ".
+    iMod ("H" with "Hσ") as "(%Hreducible & H)".
+    iModIntro. iSplit; first iSteps. iIntros "%e' %σ' %es %Hstep".
+    iApply ("H" with "[%]").
+    naive_solver.
+  Qed.
+  Lemma bwp_lift_base_step_nofork e tid E Φ :
+    to_val e = None →
+    ( ∀ nt σ κ κs,
+      state_interp nt σ (κ ++ κs) -∗
+        |={E, ∅}=>
+        ⌜base_reducible tid e σ⌝ ∗
+          ∀ e' σ' es,
+          ⌜base_step tid e σ κ e' σ' es⌝ -∗
+          £ 1 -∗
+            |={∅}=> ▷ |={∅, E}=>
+            ⌜es = []⌝ ∗
+            state_interp nt σ' κs ∗
+            BWP e' ∶ tid @ E {{ Φ }}
+    ) ⊢
+    BWP e ∶ tid @ E {{ Φ }}.
+  Proof.
+    iIntros "%He H".
+    iApply bwp_lift_base_step; first done. iIntros "%nt %σ %κ %κs Hσ".
+    iMod ("H" with "Hσ") as "($ & H)".
+    iIntros "!> %e' %σ' %es %Hstep H£".
+    iMod ("H" with "[//] H£") as "H".
+    do 2 iModIntro.
+    iMod "H" as "(-> & Hσ & H)".
+    rewrite Nat.add_0_r. iSteps.
+  Qed.
+
+  Lemma bwp_lift_atomic_base_step e tid E1 E2 Φ :
+    to_val e = None →
+    ( ∀ nt σ κ κs,
+      state_interp nt σ (κ ++ κs) -∗
+        |={E1}=>
+        ⌜base_reducible tid e σ⌝ ∗
+        ∀ e' σ' es,
+        ⌜base_step tid e σ κ e' σ' es⌝ -∗
+        £ 1 -∗
+          |={E1}[E2]▷=>
+          state_interp (nt + length es) σ' κs ∗
+          from_option Φ False (to_val e') ∗
+          [∗ list] i ↦ e ∈ es,
+            BWP e ∶ nt + i {{ fork_post }}
+    ) ⊢
+    BWP e ∶ tid @ E1 {{ Φ }}.
+  Proof.
+    iIntros "%He H".
+    iApply bwp_lift_atomic_step; first done. iIntros "%nt %σ %κ %κs Hσ".
+    iMod ("H" with "Hσ") as "(%Hreducible & H)".
+    iModIntro. iSplit; first iSteps. iIntros "%e' %σ' %es %Hstep".
+    iApply ("H" with "[%]").
+    naive_solver.
+  Qed.
+  Lemma bwp_lift_atomic_base_step_nofork e tid E1 E2 Φ :
+    to_val e = None →
+    ( ∀ nt σ κ κs,
+      state_interp nt σ (κ ++ κs) -∗
+        |={E1}=>
+        ⌜base_reducible tid e σ⌝ ∗
+          ∀ e' σ' es,
+          ⌜base_step tid e σ κ e' σ' es⌝ -∗
+          £ 1 -∗
+            |={E1}[E2]▷=>
+            ⌜es = []⌝ ∗
+            state_interp nt σ' κs ∗
+            from_option Φ False (to_val e')
+    ) ⊢
+    BWP e ∶ tid @ E1 {{ Φ }}.
+  Proof.
+    iIntros "%He H".
+    iApply bwp_lift_atomic_base_step; first done. iIntros "%nt %σ %κ %κs Hσ".
+    iMod ("H" with "Hσ") as "($ & H)".
+    iIntros "!> %e' %σ' %es %Hstep H£".
+    iMod ("H" with "[//] H£") as "H".
+    do 2 iModIntro.
+    iMod "H" as "(-> & Hσ & H)".
+    rewrite Nat.add_0_r. iSteps.
+  Qed.
+
+  Lemma bwp_lift_pure_base_step_nofork `{!Inhabited (state Λ)} e tid E1 E2 Φ :
+    ( ∀ σ,
+      base_reducible tid e σ
+    ) →
+    ( ∀ σ κ e' σ' es,
+      base_step tid e σ κ e' σ' es →
+        κ = [] ∧
+        σ' = σ ∧
+        es = []
+    ) →
+    ( |={E1}[E2]▷=>
+      ∀ σ e' κ es,
+      ⌜base_step tid e σ κ e' σ es⌝ -∗
+      £ 1 -∗
+      BWP e' ∶ tid @ E1 {{ Φ }}
+    ) ⊢
+    BWP e ∶ tid @ E1 {{ Φ }}.
+  Proof.
+    iIntros "%Hsafe %Hpure H".
+    iApply bwp_lift_pure_step_nofork; [eauto.. |].
+    iMod "H" as "H".
+    iIntros "!> !>".
+    iMod "H".
+    iIntros "!> %σ %e' %κ %es %Hstep H£".
+    iApply ("H" with "[%] H£"); first eauto.
+  Qed.
+
+  Lemma bwp_lift_pure_det_base_step_nofork `{!Inhabited (state Λ)} e1 e2 tid E1 E2 Φ :
+    ( ∀ σ1,
+      base_reducible tid e1 σ1
+    ) →
+    ( ∀ σ1 κ e2' σ2 es,
+      base_step tid e1 σ1 κ e2' σ2 es →
+        κ = [] ∧
+        σ2 = σ1 ∧
+        e2' = e2 ∧
+        es = []
+    ) →
+    ( |={E1}[E2]▷=>
+      £ 1 -∗
+      BWP e2 ∶ tid @ E1 {{ Φ }}
+    ) ⊢
+    BWP e1 ∶ tid @ E1 {{ Φ }}.
+  Proof.
+    iIntros "%Hsafe %Hpure H".
+    iApply bwp_lift_pure_det_step_nofork; [eauto.. |].
+    iSteps.
+  Qed.
+End iris_G.
