theories/zoo/program_logic/adequacy.v
@@ -15,15 +15,16 @@ Implicit Types e : expr.
 Implicit Types v : val.
 Implicit Types σ : state.
 
-Definition zoo_adequacy Σ `{zoo_Gpre : !ZooGpre Σ} e σ :
+Definition zoo_adequacy Σ `{zoo_Gpre : !ZooGpre Σ} e tid σ :
+  (if tid is Some tid then tid = 0 else True) →
   ( ∀ `{zoo_G : !ZooG Σ},
-    ⊢ WP e {{ v, True }}
+    ⊢ WP e ∷ tid {{ v, True }}
   ) →
   safe ([e], σ).
 Proof.
-  intros Hwp.
-  apply: wp_adequacy => Hinv_G κs.
-  iMod zoo_init' as "(%zoo_G & Hσ)".
+  intros Htid Hwp.
+  apply: wp_adequacy => // Hinv_G κs.
+  iMod (zoo_init' σ κs) as "(%zoo_G & Hσ)".
   iExists zoo_state_interp. repeat iExists _. iFrame.
   iApply (Hwp (Build_ZooG _)).
 Qed.
