theories/zoo/program_logic/wp.v
@@ -1,7 +1,7 @@
 From zoo Require Import
   prelude.
 From zoo.iris.program_logic Require Import
-  wp_lifting.
+  wp.
 From zoo.iris Require Import
   diaframe.
 From zoo.language Require Import
@@ -22,11 +22,16 @@ Implicit Types es : list expr.
 Implicit Types v w : val.
 Implicit Types σ : state.
 Implicit Types κ : list observation.
+Implicit Types K : ectx.
+
+#[local] Ltac wp_unseal :=
+  rewrite wp.wp_unseal /wp.wp_def;
+  select (option thread_id) (fun tid => destruct tid).
 
 Section zoo_G.
   Context `{zoo_G : !ZooG Σ}.
 
-  Lemma wp_equal v1 v2 E Φ :
+  Lemma wp_equal v1 v2 tid E Φ :
     ▷ (
       ( ⌜v1 ≉ v2⌝ -∗
         Φ #false
@@ -35,10 +40,11 @@ Section zoo_G.
         Φ #true
       )
     ) ⊢
-    WP v1 == v2 @ E {{ Φ }}.
+    WP v1 == v2 ∷ tid @ E {{ Φ }}.
   Proof.
     iIntros "HΦ".
-    iApply wp_lift_atomic_base_step_nofork; first done. iIntros "%nt %σ1 %κ %κs Hσ !>".
+    iApply bwp_wp. iIntros.
+    iApply bwp_lift_atomic_base_step_nofork; first done. iIntros "%nt %σ1 %κ %κs Hσ !>".
     iSplit. { iPureIntro. apply base_reducible_equal. }
     iIntros "%e2 %σ2 %es %Hstep _ !> !> !>".
     invert_base_step.
@@ -48,13 +54,13 @@ Section zoo_G.
       iSteps.
   Qed.
 
-  Lemma wp_alloc (tag : Z) n E :
+  Lemma wp_alloc (tag : Z) n tid E :
     (0 ≤ tag)%Z →
     (0 ≤ n)%Z →
     {{{
       True
     }}}
-      Alloc #tag #n @ E
+      Alloc #tag #n ∷ tid @ E
     {{{ l,
       RET #l;
       l ↦ₕ Header ₊tag ₊n ∗
@@ -64,7 +70,8 @@ Section zoo_G.
   Proof.
     iIntros "%Htag %Hn %Φ _ HΦ".
     Z_to_nat tag. rewrite Nat2Z.id.
-    iApply wp_lift_atomic_base_step_nofork; first done. iIntros "%nt %σ1 %κ %κs Hσ !>".
+    iApply bwp_wp. iIntros.
+    iApply bwp_lift_atomic_base_step_nofork; first done. iIntros "%nt %σ1 %κ %κs Hσ !>".
     iSplit; first auto with zoo. iIntros "%e2 %σ2 %es %Hstep _ !> !>".
     invert_base_step.
     iMod (state_interp_alloc _ _ (replicate ₊n ()%V) with "Hσ") as "(Hσ & Hheader & Hmeta & Hl)".
@@ -72,13 +79,13 @@ Section zoo_G.
     iSteps.
   Qed.
 
-  Lemma wp_block_mutable {es tag} vs E :
+  Lemma wp_block_mutable {es tag} vs tid E :
     0 < length es →
     to_vals es = Some vs →
     {{{
       True
     }}}
-      Block Mutable tag es @ E
+      Block Mutable tag es ∷ tid @ E
     {{{ l,
       RET #l;
       l ↦ₕ Header tag (length es) ∗
@@ -87,7 +94,8 @@ Section zoo_G.
     }}}.
   Proof.
     iIntros (Hlen <-%of_to_vals) "%Φ _ HΦ".
-    iApply wp_lift_atomic_base_step_nofork; first done. iIntros "%nt %σ1 %κ %κs Hσ !>".
+    iApply bwp_wp. iIntros.
+    iApply bwp_lift_atomic_base_step_nofork; first done. iIntros "%nt %σ1 %κ %κs Hσ !>".
     iSplit; first auto with zoo. iIntros "%e2 %σ2 %es %Hstep _ !> !>".
     invert_base_step.
     iMod (state_interp_alloc with "Hσ") as "(Hσ & Hheader & Hmeta & Hl)".
@@ -95,46 +103,83 @@ Section zoo_G.
     iSteps.
   Qed.
 
-  Lemma wp_block_generative {es tag} vs E :
+  Lemma wp_block_generative {es tag} vs tid E :
     to_vals es = Some vs →
     {{{
       True
     }}}
-      Block ImmutableGenerativeStrong tag es @ E
+      Block ImmutableGenerativeStrong tag es ∷ tid @ E
     {{{ bid,
       RET ValBlock (Generative (Some bid)) tag vs;
       True
     }}}.
   Proof.
     iIntros (<-%of_to_vals) "%Φ _ HΦ".
-    iApply wp_lift_atomic_base_step_nofork; first done. iIntros "%nt %σ1 %κ %κs Hσ !>".
+    iApply bwp_wp. iIntros.
+    iApply bwp_lift_atomic_base_step_nofork; first done. iIntros "%nt %σ1 %κ %κs Hσ !>".
     iSplit; first auto with zoo. iIntros "%e2 %σ2 %es %Hstep _ !> !>".
     invert_base_step.
     iSteps.
   Qed.
 
-  Lemma wp_match l hdr x_fb e_fb brs e E Φ :
+  Lemma bwp_match l hdr x_fb e_fb brs e tid E Φ :
     eval_match hdr.(header_tag) hdr.(header_size) (inl l) x_fb e_fb brs = Some e →
     ▷ l ↦ₕ hdr -∗
-    ▷ WP e @ E {{ Φ }} -∗
-    WP Match #l x_fb e_fb brs @ E {{ Φ }}.
+    ▷ BWP e ∶ tid @ E {{ Φ }} -∗
+    BWP Match #l x_fb e_fb brs ∶ tid @ E {{ Φ }}.
   Proof.
     iIntros "%He >#Hl H".
-    iApply wp_lift_base_step_nofork; first done. iIntros "%nt %σ1 %κ %κs Hσ".
+    iApply bwp_lift_base_step_nofork; first done. iIntros "%nt %σ1 %κ %κs Hσ".
     iApply fupd_mask_intro; first set_solver. iIntros "Hclose".
     iDestruct (state_interp_has_header_valid with "Hσ Hl") as %Hheaders_lookup.
     iSplit; first eauto with zoo. iIntros "%_e %_σ %es %Hstep _ !>".
     invert_base_step.
     iSteps.
   Qed.
+  Lemma bwp_match_fill K l hdr x_fb e_fb brs e tid E Φ :
+    eval_match hdr.(header_tag) hdr.(header_size) (inl l) x_fb e_fb brs = Some e →
+    ▷ l ↦ₕ hdr -∗
+    ▷ BWP fill K e ∶ tid @ E {{ Φ }} -∗
+    BWP fill K (Match #l x_fb e_fb brs) ∶ tid @ E {{ Φ }}.
+  Proof.
+    iIntros "%He Hl H".
+    iApply bwp_bind.
+    iApply (bwp_match with "Hl"); first done.
+    iApply (bwp_bind_inv with "H").
+  Qed.
+  Lemma wp_match l hdr x_fb e_fb brs e tid E Φ :
+    eval_match hdr.(header_tag) hdr.(header_size) (inl l) x_fb e_fb brs = Some e →
+    ▷ l ↦ₕ hdr -∗
+    ▷ WP e ∷ tid @ E {{ Φ }} -∗
+    WP Match #l x_fb e_fb brs ∷ tid @ E {{ Φ }}.
+  Proof.
+    wp_unseal.
+    - apply bwp_match.
+    - iIntros "%He >#Hl H %tid".
+      iSpecialize ("H" $! tid).
+      iApply (bwp_match with "Hl H"); first done.
+  Qed.
+  Lemma wp_match_fill K l hdr x_fb e_fb brs e tid E Φ :
+    eval_match hdr.(header_tag) hdr.(header_size) (inl l) x_fb e_fb brs = Some e →
+    ▷ l ↦ₕ hdr -∗
+    ▷ WP fill K e ∷ tid @ E {{ Φ }} -∗
+    WP fill K (Match #l x_fb e_fb brs) ∷ tid @ E {{ Φ }}.
+  Proof.
+    wp_unseal.
+    - apply bwp_match_fill.
+    - iIntros "%He >#Hl H %tid".
+      iSpecialize ("H" $! tid).
+      iApply (bwp_match_fill with "Hl H"); first done.
+  Qed.
 
-  Lemma wp_get_tag l hdr E Φ :
+  Lemma wp_get_tag l hdr tid E Φ :
     ▷ l ↦ₕ hdr -∗
     ▷ Φ #hdr.(header_tag) -∗
-    WP GetTag #l @ E {{ Φ }}.
+    WP GetTag #l ∷ tid @ E {{ Φ }}.
   Proof.
     iIntros ">Hheader HΦ".
-    iApply wp_lift_atomic_base_step_nofork; first done. iIntros "%nt %σ1 %κ %κs Hσ".
+    iApply bwp_wp. iIntros.
+    iApply bwp_lift_atomic_base_step_nofork; first done. iIntros "%nt %σ1 %κ %κs Hσ".
     iApply fupd_mask_intro; first set_solver. iIntros "Hclose".
     iDestruct (state_interp_has_header_valid with "Hσ Hheader") as %Hheaders_lookup.
     iSplit; first eauto with zoo. iIntros "%e %σ2 %es %Hstep _ !>".
@@ -142,13 +187,14 @@ Section zoo_G.
     iSteps.
   Qed.
 
-  Lemma wp_get_size l hdr E Φ :
+  Lemma wp_get_size l hdr tid E Φ :
     ▷ l ↦ₕ hdr -∗
     ▷ Φ #hdr.(header_size) -∗
-    WP GetSize #l @ E {{ Φ }}.
+    WP GetSize #l ∷ tid @ E {{ Φ }}.
   Proof.
     iIntros ">Hheader HΦ".
-    iApply wp_lift_atomic_base_step_nofork; first done. iIntros "%nt %σ1 %κ %κs Hσ".
+    iApply bwp_wp. iIntros.
+    iApply bwp_lift_atomic_base_step_nofork; first done. iIntros "%nt %σ1 %κ %κs Hσ".
     iApply fupd_mask_intro; first set_solver. iIntros "Hclose".
     iDestruct (state_interp_has_header_valid with "Hσ Hheader") as %Hheaders_lookup.
     iSplit; first eauto with zoo. iIntros "%e %σ2 %es %Hstep _ !>".
@@ -156,36 +202,38 @@ Section zoo_G.
     iSteps.
   Qed.
 
-  Lemma wp_load l fld dq v E :
+  Lemma wp_load l fld dq v tid E :
     {{{
       ▷ (l +ₗ fld) ↦{dq} v
     }}}
-      Load #l #fld @ E
+      Load #l #fld ∷ tid @ E
     {{{
       RET v;
       (l +ₗ fld) ↦{dq} v
     }}}.
   Proof.
     iIntros "%Φ >Hl HΦ".
-    iApply wp_lift_atomic_base_step_nofork; first done. iIntros "%nt %σ1 %κ %κs Hσ !>".
+    iApply bwp_wp. iIntros.
+    iApply bwp_lift_atomic_base_step_nofork; first done. iIntros "%nt %σ1 %κ %κs Hσ !>".
     iDestruct (state_interp_pointsto_valid with "Hσ Hl") as %Hlookup.
     iSplit; first eauto with zoo. iIntros "%e2 %σ2 %es %Hstep _ !> !> !>".
     invert_base_step.
     iSteps.
   Qed.
 
-  Lemma wp_store l fld w v E :
+  Lemma wp_store l fld w v tid E :
     {{{
       ▷ (l +ₗ fld) ↦ w
     }}}
-      Store #l #fld v @ E
+      Store #l #fld v ∷ tid @ E
     {{{
       RET ();
       (l +ₗ fld) ↦ v
     }}}.
   Proof.
     iIntros "%Φ >Hl HΦ".
-    iApply wp_lift_atomic_base_step_nofork; first done. iIntros "%nt %σ1 %κ %κs Hσ !>".
+    iApply bwp_wp. iIntros.
+    iApply bwp_lift_atomic_base_step_nofork; first done. iIntros "%nt %σ1 %κ %κs Hσ !>".
     iDestruct (state_interp_pointsto_valid with "Hσ Hl") as %Hlookup.
     iSplit; first eauto with zoo. iIntros "%e2 %σ2 %es %Hstep _ !> !>".
     invert_base_step.
@@ -193,18 +241,19 @@ Section zoo_G.
     iSteps.
   Qed.
 
-  Lemma wp_xchg l fld w v E :
+  Lemma wp_xchg l fld w v tid E :
     {{{
       ▷ (l +ₗ fld) ↦ w
     }}}
-      Xchg (#l, #fld)%V v @ E
+      Xchg (#l, #fld)%V v ∷ tid @ E
     {{{
       RET w;
       (l +ₗ fld) ↦ v
     }}}.
   Proof.
     iIntros "%Φ >Hl HΦ".
-    iApply wp_lift_atomic_base_step_nofork; first done. iIntros "%nt %σ1 %κ %κs Hσ !>".
+    iApply bwp_wp. iIntros.
+    iApply bwp_lift_atomic_base_step_nofork; first done. iIntros "%nt %σ1 %κ %κs Hσ !>".
     iDestruct (state_interp_pointsto_valid with "Hσ Hl") as %Hlookup.
     iSplit; first eauto with zoo. iIntros "%e2 %σ2 %es %Hstep _ !> !>".
     invert_base_step.
@@ -212,7 +261,7 @@ Section zoo_G.
     iSteps.
   Qed.
 
-  Lemma wp_cas l fld dq v v1 v2 E Φ :
+  Lemma wp_cas l fld dq v v1 v2 tid E Φ :
     ▷ (l +ₗ fld) ↦{dq} v -∗
     ▷ (
       ( ⌜v ≉ v1⌝ -∗
@@ -228,10 +277,11 @@ Section zoo_G.
           )
       )
     ) -∗
-    WP CAS (#l, #fld)%V v1 v2 @ E {{ Φ }}.
+    WP CAS (#l, #fld)%V v1 v2 ∷ tid @ E {{ Φ }}.
   Proof.
     iIntros ">Hl HΦ".
-    iApply wp_lift_atomic_base_step_nofork; first done. iIntros "%nt %σ1 %κ %κs Hσ !>".
+    iApply bwp_wp. iIntros.
+    iApply bwp_lift_atomic_base_step_nofork; first done. iIntros "%nt %σ1 %κ %κs Hσ !>".
     iDestruct (state_interp_pointsto_valid with "Hσ Hl") as %Hlookup.
     iSplit. { iPureIntro. eapply base_reducible_cas. done. }
     iIntros "%e2 %σ2 %es %Hstep _ !> !>".
@@ -243,13 +293,13 @@ Section zoo_G.
       iMod (state_interp_pointsto_update with "Hσ Hl") as "($ & Hl)".
       iSteps.
   Qed.
-  Lemma wp_cas_suc l fld lit lit1 v2 E :
+  Lemma wp_cas_suc l fld lit lit1 v2 tid E :
     literal_physical lit →
     lit = lit1 →
     {{{
       ▷ (l +ₗ fld) ↦ #lit
     }}}
-      CAS (#l, #fld)%V #lit1 v2 @ E
+      CAS (#l, #fld)%V #lit1 v2 ∷ tid @ E
     {{{
       RET #true;
       (l +ₗ fld) ↦ v2
@@ -260,18 +310,19 @@ Section zoo_G.
     destruct lit; [iSteps.. | done | done].
   Qed.
 
-  Lemma wp_faa l fld (i1 i2 : Z) E :
+  Lemma wp_faa l fld (i1 i2 : Z) tid E :
     {{{
       ▷ (l +ₗ fld) ↦ #i1
     }}}
-      FAA (#l, #fld)%V #i2 @ E
+      FAA (#l, #fld)%V #i2 ∷ tid @ E
     {{{
       RET #i1;
       (l +ₗ fld) ↦ #(i1 + i2)
     }}}.
   Proof.
     iIntros "%Φ >Hl HΦ".
-    iApply wp_lift_atomic_base_step_nofork; first done. iIntros "%nt %σ1 %κ %κs Hσ !>".
+    iApply bwp_wp. iIntros.
+    iApply bwp_lift_atomic_base_step_nofork; first done. iIntros "%nt %σ1 %κ %κs Hσ !>".
     iDestruct (state_interp_pointsto_valid with "Hσ Hl") as %Hlookup.
     iSplit; first eauto with zoo. iIntros "%e2 %σ2 %es %Hstep _ !> !>".
     invert_base_step.
@@ -279,50 +330,53 @@ Section zoo_G.
     iSteps.
   Qed.
 
-  Lemma wp_fork e E Φ :
-    ▷ WP e @ ⊤ {{ _, True }} -∗
+  Lemma wp_fork e tid E Φ :
+    ▷ WP e {{ _, True }} -∗
     ▷ Φ ()%V -∗
-    WP Fork e @ E {{ Φ }}.
+    WP Fork e ∷ tid @ E {{ Φ }}.
   Proof.
     iIntros "H HΦ".
-    iApply wp_lift_atomic_base_step; first done. iIntros "%nt %σ1 %κ %κs Hσ !>".
+    iApply bwp_wp. iIntros.
+    iApply bwp_lift_atomic_base_step; first done. iIntros "%nt %σ1 %κ %κs Hσ !>".
     iSplit; first auto with zoo. iIntros "%v2 %σ2 %es %Hstep _ !> !> !>".
     invert_base_step.
+    iDestruct (wp_bwp with "H") as "$".
     iSteps.
   Qed.
 
-  Lemma wp_proph E :
+  Lemma wp_proph tid E :
     {{{
       True
     }}}
-      Proph @ E
+      Proph ∷ tid @ E
     {{{ prophs pid,
       RET #pid;
       prophet_model' pid prophs
     }}}.
   Proof.
     iIntros "%Φ _ HΦ".
-    iApply wp_lift_atomic_base_step_nofork; first done. iIntros "%nt %σ1 %κ %κs Hσ !>".
+    iApply bwp_wp. iIntros.
+    iApply bwp_lift_atomic_base_step_nofork; first done. iIntros "%nt %σ1 %κ %κs Hσ !>".
     iSplit; first eauto with zoo. iIntros "%e2 %σ2 %es %Hstep _ !> !>".
     invert_base_step.
     iMod (state_interp_prophet_new with "Hσ") as "(%prophs & Hσ & Hpid)"; first done.
     iSteps.
   Qed.
 
-  Lemma wp_resolve e pid v prophs E Φ :
+  Lemma bwp_resolve e pid v prophs tid E Φ :
     Atomic e →
     to_val e = None →
     prophet_model' pid prophs -∗
-    WP e @ E {{ res,
+    BWP e ∶ tid @ E {{ res,
       ∀ prophs',
       ⌜prophs = (res, v) :: prophs'⌝ -∗
       prophet_model' pid prophs' -∗
       Φ res
     }} -∗
-    WP Resolve e #pid v @ E {{ Φ }}.
+    BWP Resolve e #pid v ∶ tid @ E {{ Φ }}.
   Proof.
     iIntros "%Hatomic %He Hpid H".
-    rewrite !wp_unfold /wp_pre /= He. simpl in *.
+    rewrite !bwp_unfold /bwp_pre /= He. simpl in *.
     iIntros "%nt %σ1 %κ %κs Hσ".
     destruct κ as [| (pid' & (w' & v')) κ' _] using rev_ind.
     - iMod ("H" with "Hσ") as "(%Hreducible & H)".
@@ -342,8 +396,26 @@ Section zoo_G.
       do 2 iModIntro.
       iMod "H" as "(Hσ & H)".
       iMod (state_interp_prophet_resolve with "Hσ Hpid") as "(%prophs' & -> & $ & Hpid')".
-      rewrite !wp_unfold /wp_pre /=.
+      rewrite !bwp_unfold /bwp_pre /=.
       iDestruct "H" as "(HΦ & $)".
       iSteps.
+  Qed.
+  Lemma wp_resolve e pid v prophs tid E Φ :
+    Atomic e →
+    to_val e = None →
+    prophet_model' pid prophs -∗
+    WP e ∷ tid @ E {{ res,
+      ∀ prophs',
+      ⌜prophs = (res, v) :: prophs'⌝ -∗
+      prophet_model' pid prophs' -∗
+      Φ res
+    }} -∗
+    WP Resolve e #pid v ∷ tid @ E {{ Φ }}.
+  Proof.
+    wp_unseal.
+    - apply bwp_resolve.
+    - iIntros "%Hatomic %He Hpid H %tid".
+      iSpecialize ("H" $! tid).
+      iApply (bwp_resolve with "Hpid H"); first done.
   Qed.
 End zoo_G.
