theories/zoo_kcas/kcas_1.v
@@ -1346,7 +1346,7 @@ Section kcas_1_G.
       wp_load. wp_pures.
 
       wp_bind (Resolve _ _ _).
-      wp_apply (wp_wand _ _ (λ res,
+      wp_apply (wp_wand (λ res,
         ∃ b,
         ⌜res = #b⌝ ∗
         ⌜b = true → final_status_to_bool fstatus = metadata_success η⌝ ∗
@@ -1482,7 +1482,7 @@ Section kcas_1_G.
       }
 
       wp_bind (if: _ then _ else _)%E.
-      wp_apply (wp_wand _ _ itype_unit with "[- HΦ]") as (res) "->".
+      wp_apply (wp_wand itype_unit with "[- HΦ]") as (res) "->".
       { destruct b; last iSteps.
         wp_smart_apply (kcas_1_clear_spec with "[$Hcasn_inv' $Hlstatus_lb]"); first auto.
         iSteps.
